@prefix : <http://visualdataweb.org/SpaceScience/> .
@prefix dc: <http://purl.org/dc/elements/1.1/> .
@prefix vs: <http://www.w3.org/2003/06/sw-vocab-status/ns#> .
@prefix owl: <http://www.w3.org/2002/07/owl#> .
@prefix rdf: <http://www.w3.org/1999/02/22-rdf-syntax-ns#> .
@prefix wot: <http://xmlns.com/wot/0.1/> .
@prefix xml: <http://www.w3.org/XML/1998/namespace> .
@prefix xsd: <http://www.w3.org/2001/XMLSchema#> .
@prefix foaf: <http://xmlns.com/foaf/0.1/> .
@prefix rdfs: <http://www.w3.org/2000/01/rdf-schema#> .
@base <http://visualdataweb.org/SpaceScience/> .

<http://visualdataweb.org/SpaceScience/> rdf:type owl:Ontology ;
                                          dc:creator "Sanjeev Sun Shakya" ;
                                          dc:description "Space Science Knowledge Graph"@en ;
                                          dc:title "Space Science"@en ;
                                          owl:versionInfo "1.1"@en .

#################################################################
#    Annotation properties
#################################################################

###  http://purl.org/dc/elements/1.1/creator
dc:creator rdf:type owl:AnnotationProperty .


###  http://purl.org/dc/elements/1.1/description
dc:description rdf:type owl:AnnotationProperty .


###  http://purl.org/dc/elements/1.1/title
dc:title rdf:type owl:AnnotationProperty .


#################################################################
#    Classes
#################################################################

###  http://visualdataweb.org/SpaceScience/Active
:Active rdf:type owl:Class ;
        rdfs:subClassOf :Galaxy ;
        owl:disjointWith :Normal ;
        rdfs:comment """Definition: In an active galaxy, its supermassive black hole is accreting material from the galaxy's dense central region.

Source: https://imagine.gsfc.nasa.gov/science/objects/active_galaxies1.html#:~:text=Most%2C%20if%20not%20all%2C%20normal,and%20form%20into%20a%20disk.

Justification: Classification of active galaxies is difficult, historically contingent, and subject to change, and recent work indicates that at least some classes of
active galaxies may be one and the same kind of object viewed at different angles from Earth. On the principle that physical nature rather than accidental viewing angle from Earth should be one of the chief criteria for class status, if such a “unified theory” of active galaxies is demonstrated.""" .


###  http://visualdataweb.org/SpaceScience/Advanced
:Advanced rdf:type owl:Class ;
          rdfs:subClassOf :G_Interacting .


###  http://visualdataweb.org/SpaceScience/Alidade
:Alidade rdf:type owl:Class ;
         rdfs:subClassOf :Observational ;
         rdfs:comment """Definition: a device that allows one to sight a distant object and use the line of sight to perform a task

Source: https://en.wikipedia.org/wiki/Alidade""" .


###  http://visualdataweb.org/SpaceScience/Anomalous_Cosmic_Ray
:Anomalous_Cosmic_Ray rdf:type owl:Class ;
                      rdfs:subClassOf :Energetic_Particles ;
                      owl:disjointWith :Solar_Wind ;
                      rdfs:seeAlso """Definitions: Anomalous cosmic rays (ACRs) are energetic particles of interstellar
origin that travel into the Solar System near the speed of light.
They have energies of about one thousand electron volts (one KeV,
ten times the solar wind energies) to 350 million electron volts
(350 MeV).

Source: Classifying the Cosmos (Book)""" .


###  http://visualdataweb.org/SpaceScience/Armillary_sphere
:Armillary_sphere rdf:type owl:Class ;
                  rdfs:subClassOf :Observational ;
                  rdfs:comment """Definition: An armillary sphere (variations are known as spherical astrolabe, armilla, or armil) is a model of objects in the sky (on the celestial sphere), consisting of a spherical framework of rings, centered on Earth or the Sun, that represent lines of celestial longitude and latitude and other astronomically important features, such as the ecliptic.

Source: https://en.wikipedia.org/wiki/Armillary_sphere""" .


###  http://visualdataweb.org/SpaceScience/Association
:Association rdf:type owl:Class ;
             rdfs:subClassOf :Star_Systems ;
             rdfs:comment """Definition: An association of stars is a group of tens to hundreds of young
stars that are close together because they were formed from the
same giant molecular cloud.""" .


###  http://visualdataweb.org/SpaceScience/Asteroid
:Asteroid rdf:type owl:Class ;
          rdfs:subClassOf :Small_Bodies_of_Solar_System ;
          rdfs:comment """Definition: A minor planet is one class of small rocky bodies of the Solar
System orbiting the Sun, as distinct from the classes of major planets
, dwarf planets, and satellites. Also known
as asteroids, they are distinguished from comets and other
small bodies of the Solar System such as trans-Neptunian objects
, as defined by the International Astronomical Union in
2006. They range in size from about 600 miles in diameter down
to pebbles.

Source: Classifying the Cosmos (Book)""" .


###  http://visualdataweb.org/SpaceScience/Asteroid_Groups
:Asteroid_Groups rdf:type owl:Class ;
                 rdfs:subClassOf :Systems ;
                 rdfs:comment """Definition: Asteroid groups are populations of minor planets with
similar orbits, probably related to their origins. While the terms
“minor planet” and “asteroid” are technically interchangeable for
individual objects, for historical reasons the latter term in practice
is usually used for groups, including the main asteroid belt
located between Mars and Jupiter.

Source: Classifying the Cosmos (Book)""" .


###  http://visualdataweb.org/SpaceScience/Astrolabe
:Astrolabe rdf:type owl:Class ;
           rdfs:subClassOf :Observational ;
           rdfs:comment """Definitions: It is an ancient astronomical instrument that was a handheld model of the universe

Source: https://en.wikipedia.org/wiki/Astrolabe""" .


###  http://visualdataweb.org/SpaceScience/Astrometric
:Astrometric rdf:type owl:Class ;
             rdfs:subClassOf :Binary ;
             rdfs:comment """Definition: distinguished by positional changes

Source: Classifying the Cosmos (Book)""" .


###  http://visualdataweb.org/SpaceScience/Astronomical_Instruments
:Astronomical_Instruments rdf:type owl:Class ;
                          rdfs:subClassOf :Astronomy ;
                          rdfs:comment """Definition: An astronomical instrument generally refers to a type of equipment used for the study, observation, or measurement of celestial objects.

Source: https://www.allthescience.org/what-are-the-different-types-of-astronomical-instruments.htm

Justification: Instruments used to study astromony based where it is used either earth or outer space.""" .


###  http://visualdataweb.org/SpaceScience/Astronomical_Objects
:Astronomical_Objects rdf:type owl:Class ;
                      rdfs:subClassOf :Astronomy ;
                      rdfs:comment """Category: An astronomical object or celestial object is a naturally occurring physical entity, association, or structure that exists in the observable universe.

Source: https://en.wikipedia.org/wiki/Astronomical_object

Justification: Classifciation based on the gravity as gravity is the determining factor for the structure and organization of planets, stars, and galaxies, their families, and classes of objects.

Gravity is the dominant force at work in astronomical protosystems, as planets, stars, and galaxies form—by different mechanisms to be sure, but all subject to the laws of gravity as delineated by Newton.""" ;
                      rdfs:label "Astronomical Objects"@en ,
                                 "Astronomical_Objects"@iri-based .


###  http://visualdataweb.org/SpaceScience/Astronomical_Phenomena
:Astronomical_Phenomena rdf:type owl:Class ;
                        rdfs:subClassOf :Astronomy ;
                        rdfs:comment """Category: Aggregates of matter in outer space, such as stars, planets, comets, etc. and the properties and processes they undergo.

Source: https://www.definitions.net/definition/astronomical+phenomena#:~:text=Library%20of%20Medicine-,Astronomical%20Phenomena,properties%20and%20processes%20they%20undergo.

Justification: Classification based on where it occurs, either within the solar system or outside the solar system""" ;
                        rdfs:label "Astronomical Phenomena"@en ,
                                   "Astronomical_Phenomena"@iri-based .


###  http://visualdataweb.org/SpaceScience/Astronomy
:Astronomy rdf:type owl:Class ;
           rdfs:label "Astronomy"@en ,
                      "Astronomy"@iri-based ,
                      "Space_Science"@iri-based .


###  http://visualdataweb.org/SpaceScience/Aurora
:Aurora rdf:type owl:Class ;
        rdfs:subClassOf :Single_Objects ;
        rdfs:comment """Definition: An aurora, also commonly known as the polar lights, is a natural light display in Earth's sky, predominantly seen in high-latitude regions (around the Arctic and Antarctic). Auroras display dynamic patterns of brilliant lights that appear as curtains, rays, spirals, or dynamic flickers covering the entire sky.

Source: https://en.wikipedia.org/wiki/Aurora

Justification: Classification based on the where it is observed from Earth.""" ;
        rdfs:label "Aurora"@en .


###  http://visualdataweb.org/SpaceScience/Aurora_australis
:Aurora_australis rdf:type owl:Class ;
                  rdfs:subClassOf :Aurora ;
                  rdfs:comment "Definition: It is observed from the Southern part of Earth" ;
                  rdfs:label "Aurora australis"@en .


###  http://visualdataweb.org/SpaceScience/Aurora_borealis
:Aurora_borealis rdf:type owl:Class ;
                 rdfs:subClassOf :Aurora ;
                 rdfs:comment "Definition: Definition: It is observed from the Northern part of Earth" ;
                 rdfs:label "Aurora borealis"@en .


###  http://visualdataweb.org/SpaceScience/Binary
:Binary rdf:type owl:Class ;
        rdfs:subClassOf :Star_Systems ;
        rdfs:comment """Definition: Binary stars are two stars that are
gravitationally bound in a mutual orbit. They are sometimes also
termed double stars, but that designation may also include stars
that only appear close together in the sky.

Source: Classifying the Cosmos (Book)

Justification: Classification based on method of observation.""" .


###  http://visualdataweb.org/SpaceScience/Black_Hole
:Black_Hole rdf:type owl:Class ;
            rdfs:subClassOf :Evolutionary_Endpoints ;
            rdfs:comment """Definition: A black hole is an infinitely dense region of space with a gravitational
field so intense that even light cannot escape.

Source: Classifying the Cosmos (Book)

Justification: Classification based on the their masses relative to the Sun.""" .


###  http://visualdataweb.org/SpaceScience/Blazar
:Blazar rdf:type owl:Class ;
        rdfs:subClassOf :Active ;
        rdfs:comment """Definition: Blazars are active galactic nuclei viewed head-on, made visible by
their relativistic jets pointed directly at us. They vary frequently,
erratically, and rapidly at an array of wavelengths, with their
luminosity fluctuating by more than ten times, and by 10 to 50%
in only a few hours.""" .


###  http://visualdataweb.org/SpaceScience/Blink_comparator
:Blink_comparator rdf:type owl:Class ;
                  rdfs:subClassOf :Observational ;
                  rdfs:comment """Definitions: A blink comparator is a viewing apparatus formerly used by astronomers to find differences between two photographs of the night sky.

Source: https://en.wikipedia.org/wiki/Blink_comparator""" .


###  http://visualdataweb.org/SpaceScience/Bolometer
:Bolometer rdf:type owl:Class ;
           rdfs:subClassOf :Recording ;
           rdfs:comment """Definition: A bolometer is a device for measuring radiant heat by means of a material having a temperature-dependent electrical resistance.

Source: https://en.wikipedia.org/wiki/Bolometer""" .


###  http://visualdataweb.org/SpaceScience/Bright_Giant
:Bright_Giant rdf:type owl:Class ;
              rdfs:subClassOf :Post-Main_Sequence ;
              rdfs:comment """Definition: Bright giants are luminosity class II stars intermediate between
giant  and supergiant  stars, according to the MK Yerkes
classification. Of the five classes delineated in that system, bright
giants are in some ways the least distinct, since they are brighter
than the giants of class III but in a similar state of evolution, having
exhausted their core hydrogen and started or nearly started to
undergo helium fusion.

Source: Classifying the Cosmos (Book)""" .


###  http://visualdataweb.org/SpaceScience/Brown_Dwarf
:Brown_Dwarf rdf:type owl:Class ;
             rdfs:subClassOf :Substellar ;
             rdfs:comment """Definition: Brown dwarfs are objects intermediate in mass between planets
and stars, too large to have formed as planets, too small to sustain
hydrogen fusion.

Source: Classifying the Cosmos (Book)""" .


###  http://visualdataweb.org/SpaceScience/CRM_Regular
:CRM_Regular rdf:type owl:Class ;
             rdfs:subClassOf :CR_Many_Material ;
             rdfs:comment """Definition: Objects whose shape is prior known with concavities.

Justification: Classification based on the size of the object. The size is distinguished in three different kinds, small, which is below 10cm, medium, which is between 10cm and 1.5 meter and larger than 1.5 meter in diameter.""" .


###  http://visualdataweb.org/SpaceScience/CR_Many_Material
:CR_Many_Material rdf:type owl:Class ;
                  rdfs:subClassOf :C_Regular_Spinning ;
                  rdfs:comment """Definition: Objects that are composed of multiple material. 

Justification: Classification based on the shape of the object.""" .


###  http://visualdataweb.org/SpaceScience/CSMR_Large
:CSMR_Large rdf:type owl:Class ;
            rdfs:subClassOf :CSM_Regular .


###  http://visualdataweb.org/SpaceScience/CSM_Regular
:CSM_Regular rdf:type owl:Class ;
             rdfs:subClassOf :CS_Many_Material ;
             rdfs:comment """Definition: Objects whose shape is prior known with concavities.

Justification: Classification based on the size of the object. The size is distinguished in three different kinds, small, which is below 10cm, medium, which is between 10cm and 1.5 meter and larger than 1.5 meter in diameter.""" .


###  http://visualdataweb.org/SpaceScience/CS_Many_Material
:CS_Many_Material rdf:type owl:Class ;
                  rdfs:subClassOf :C_Stable ;
                  rdfs:comment """Definition: Objects that are composed of multiple material. 

Justification: Classification based on the shape of the object.""" .


###  http://visualdataweb.org/SpaceScience/CUMR_Large
:CUMR_Large rdf:type owl:Class ;
            rdfs:subClassOf :CRM_Regular .


###  http://visualdataweb.org/SpaceScience/C_Regular_Spinning
:C_Regular_Spinning rdf:type owl:Class ;
                    rdfs:subClassOf :Controlled_Orbit ;
                    owl:disjointWith :C_Stable ;
                    rdfs:comment """Definition: Objects that are spinning normally.

Justification: Classification based on the number of material used to build the instrument.""" .


###  http://visualdataweb.org/SpaceScience/C_Stable
:C_Stable rdf:type owl:Class ;
          rdfs:subClassOf :Controlled_Orbit ;
          rdfs:comment """Definition: Objects that are stationary and stable

Justification: Classification based on the number of material used to build the instrument.""" .


###  http://visualdataweb.org/SpaceScience/Celatone
:Celatone rdf:type owl:Class ;
          rdfs:subClassOf :Recording ;
          rdfs:comment """Definition: The celatone was a device invented by Galileo Galilei to observe Jupiter's moons with the purpose of finding longitude on Earth.

Source: https://en.wikipedia.org/wiki/Celatone""" .


###  http://visualdataweb.org/SpaceScience/Celestial_sphere
:Celestial_sphere rdf:type owl:Class ;
                  rdfs:subClassOf :Observational ;
                  rdfs:comment """Definition: the celestial sphere is an abstract sphere that has an arbitrarily large radius and is concentric to Earth.

Source: https://en.wikipedia.org/wiki/Celestial_sphere""" .


###  http://visualdataweb.org/SpaceScience/Circumgalactic
:Circumgalactic rdf:type owl:Class ;
                rdfs:subClassOf :Kingdom_of_Galaxies ;
                rdfs:comment """Definition: Surrounding or occurring in the vicinity of a Galaxy

Justification: Classification based on the contituents of the object""" .


###  http://visualdataweb.org/SpaceScience/Circumplanetary
:Circumplanetary rdf:type owl:Class ;
                 rdfs:subClassOf :Kingdom_of_Planets ;
                 rdfs:comment """Definitions: Surrounding or occurring in the vicinity of a Planet

Source: https://www.merriam-webster.com/dictionary/circumplanetary#:~:text=Definition%20of%20circumplanetary,to%20a%20planet%20circumplanetary%20space

Justification: Classification based on the object's constituents and physical property.""" .


###  http://visualdataweb.org/SpaceScience/Circumstellar
:Circumstellar rdf:type owl:Class ;
               rdfs:subClassOf :Kingdom_of_Stars ;
               rdfs:comment """Definition: Surrounding or occurring in the vicinity of a star

Source: https://www.merriam-webster.com/dictionary/circumstellar

Justification: Classification based on how the object is formed.""" .


###  http://visualdataweb.org/SpaceScience/Class_I
:Class_I rdf:type owl:Class ;
         rdfs:subClassOf :Seyfert ;
         owl:disjointWith :Class_II ;
         rdfs:comment """Definition: Seyfert I galaxies exhibit both narrow and broad emission lines and are believed to be young AGNs accreting mass. They show extreme variability
compared to Seyfert II types.""" .


###  http://visualdataweb.org/SpaceScience/Class_II
:Class_II rdf:type owl:Class ;
          rdfs:subClassOf :Seyfert ;
          rdfs:comment """Definition: Class II exhibits only narrow emission lines, probably because
of its 51-degree tilt to our line of sight.""" .


###  http://visualdataweb.org/SpaceScience/Classical_KBOs
:Classical_KBOs rdf:type owl:Class ;
                rdfs:subClassOf :Kuiper_Belt ;
                rdfs:comment """Definition: composing about two-thirds of the objects
known at that time, have small eccentricities and semi-major
axes between 41 and 46 astronomical units.

Source: Classifying the Cosmos (Book)""" .


###  http://visualdataweb.org/SpaceScience/Classical_T_Tauri_stars
:Classical_T_Tauri_stars rdf:type owl:Class ;
                         rdfs:subClassOf :T-Tauri ;
                         owl:disjointWith :Weak_T_Tauri_stars ;
                         rdfs:comment """Definition: Stars with extensive disks resulting in strong emission lines

Source: Classifying the Cosmos (Book)""" .


###  http://visualdataweb.org/SpaceScience/Comet
:Comet rdf:type owl:Class ;
       rdfs:subClassOf :Small_Bodies_of_Solar_System ;
       rdfs:comment """Definition: Comets are known to be small
objects formed in the outer Solar System with nuclei composed of
ice, rock, and dust, interspersed with frozen gases and other volatiles
that sublimate (vaporize) as the comet enters the inner Solar
System, producing a coma and sometimes a spectacular tail. Their
nuclei typically range in size from 100 meters to 50 km.

Source: Classifying the Cosmos (Book)""" .


###  http://visualdataweb.org/SpaceScience/Conjunction
:Conjunction rdf:type owl:Class ;
             rdfs:subClassOf :Multiple_Objects ;
             rdfs:comment "Definition: In astronomy, a conjunction occurs when two astronomical objects or spacecraft have either the same right ascension or the same ecliptic longitude, usually as observed from Earth." .


###  http://visualdataweb.org/SpaceScience/Controlled_Orbit
:Controlled_Orbit rdf:type owl:Class ;
                  rdfs:subClassOf :Outer_Space ;
                  owl:disjointWith :UnControlled_Orbit ;
                  rdfs:comment """Definition: Objects whose movement around the orbit is controlled. 

Source: https://amostech.com/TechnicalPapers/2013/Orbital_Debris/JAH.pdf

Justification: Classification is based on the attitude state, i.e, how the attiute of the object is evolving ober time, is it actively stabilized, naturally stable, spinning mderately around one axis or spinning in irregular manner.""" .


###  http://visualdataweb.org/SpaceScience/Cool_Atomic_Cloud
:Cool_Atomic_Cloud rdf:type owl:Class ;
                   rdfs:subClassOf :S_Gas ;
                   rdfs:comment """Definition: composed mainly of cold neutral hydrogen (H I)

Source: Classifying the Cosmos (Book)""" .


###  http://visualdataweb.org/SpaceScience/Core_Collapse_Supernova_Remnant
:Core_Collapse_Supernova_Remnant rdf:type owl:Class ;
                                 rdfs:subClassOf :Circumstellar ;
                                 rdfs:comment """Definition: A supernova remnant is the remains of material
ejected during the explosion of a supernova (S 11), a process
that seeds the interstellar medium with heavy elements.

Source: Classifying the Cosmos (Book)""" .


###  http://visualdataweb.org/SpaceScience/Dark_Nebulae
:Dark_Nebulae rdf:type owl:Class ;
              rdfs:subClassOf :S_Dust ;
              owl:disjointWith :Reflection_Nebulae ;
              rdfs:comment """Definition: A dark nebula, also called an absorption nebula because the gas
component absorbs most or all of the light from the hotter star
or emission nebula behind it, is composed largely of interstellar
dust interspersed with gas.

Source: Classifying the Cosmos (Book)""" .


###  http://visualdataweb.org/SpaceScience/Debris_disk
:Debris_disk rdf:type owl:Class ;
             rdfs:subClassOf :Circumstellar ;
             rdfs:comment """Definition: Debris disks are residual materials observed around stars in the
form of a flattened disk after planet formation has taken place. As
such, this class is distinguished from protoplanetary disks, such as
proplyds that exist before planet formation, and from circumstellar
shells formed by mass loss from stars later in stellar
evolution.

Source: Classifying the Cosmos (Book)""" .


###  http://visualdataweb.org/SpaceScience/Dioptra
:Dioptra rdf:type owl:Class ;
         rdfs:subClassOf :Observational ;
         rdfs:comment """Definition: It is a classical astronomical and surveying instrument, dating from the 3rd century BC. 

Source: https://en.wikipedia.org/wiki/Dioptra""" .


###  http://visualdataweb.org/SpaceScience/Dust
:Dust rdf:type owl:Class ;
      rdfs:subClassOf :Interplanetary_Medium ;
      rdfs:comment """Definition: Interplanetary dust (IDP), sometimes called cosmic dust, consists
of particles ranging in diameter from 10 to 200 micrometers—
about the width of a single human hair.
In contrast to interplanetary gas, which is the local interstellar
medium the Solar System happens to be passing through,
most IDPs originate in the Solar System itself.

Source: Classifying the Cosmos (Book)""" .


###  http://visualdataweb.org/SpaceScience/Dwarf
:Dwarf rdf:type owl:Class ;
       rdfs:subClassOf :Main_Sequence ;
       owl:disjointWith :Subdwarf ;
       rdfs:comment """Definition: Dwarf are those stars in their
core hydrogen-burning stage, so called because they form a clear
band or “sequence” of stars when stellar absolute magnitudes or
luminosities are plotted against stellar surface temperatures.

Source:Classifying the Cosmos (Book)""" .


###  http://visualdataweb.org/SpaceScience/Dwarf_Planet
:Dwarf_Planet rdf:type owl:Class ;
              rdfs:subClassOf :Subplanetary ;
              rdfs:comment """Definition: Dwarf planet as defined by the IAU orbits the Sun, is massive
enough to be rounded by its own gravity, is not a satellite, and
has not cleared its orbit of other materials.

Source: Classifying the cosmos (Book)""" .


###  http://visualdataweb.org/SpaceScience/Early
:Early rdf:type owl:Class ;
       rdfs:subClassOf :G_Interacting .


###  http://visualdataweb.org/SpaceScience/Earth_Instrument
:Earth_Instrument rdf:type owl:Class ;
                  rdfs:subClassOf :Astronomical_Instruments ;
                  rdfs:comment """Definition: Instruments used from earth to study Astronomy

Justification: Classification based on the scope of use i.e either for Obersvational use or for recording.""" .


###  http://visualdataweb.org/SpaceScience/Ecplise
:Ecplise rdf:type owl:Class ;
         rdfs:subClassOf :Multiple_Objects ;
         rdfs:comment """Definition: An eclipse is an astronomical event that occurs when an astronomical object or spacecraft is temporarily obscured, by passing into the shadow of another body or by having another body pass between it and the viewer.
In most calendar years there are two lunar eclipses; in some years one or three or none occur. Solar eclipses occur two to five times a year, five being exceptional; there last were five in 1935, and there will not be five again until 2206. 

Source: https://en.wikipedia.org/wiki/Eclipse#:~:text=An%20eclipse%20is%20an%20astronomical,is%20known%20as%20a%20syzygy.

Justification: Classification based on the position of sun moon and earth.""" ;
         rdfs:label "Ecplises"@en ,
                    "Ecplises"@iri-based .


###  http://visualdataweb.org/SpaceScience/Elliptical
:Elliptical rdf:type owl:Class ;
            rdfs:subClassOf :Normal ;
            rdfs:comment """Definition: elliptical galaxies are almost featureless aggregations of stars distinguished by an ellipsoidal or spherical morphology.

Justification: Classification based on Luminosity.""" .


###  http://visualdataweb.org/SpaceScience/Energetic_Particles
:Energetic_Particles rdf:type owl:Class ;
                     rdfs:subClassOf :Interplanetary_Medium ;
                     rdfs:comment """Definition: Particles ranging in energy from just above solar wind, ≳1 keV, to galactic cosmic rays of many GeV or greater are observed to be always present in the interplanetary medium. These suprathermal particles appear to come from many different sources: among them the galaxy and nearby interstellar medium, the Sun, planetary magnetospheres and bow shock waves.

Source: https://link.springer.com/article/10.1007/BF00149816

Justification: Classfication based on the origin of the particles.""" .


###  http://visualdataweb.org/SpaceScience/Equatorium
:Equatorium rdf:type owl:Class ;
            rdfs:subClassOf :Recording ;
            rdfs:comment """Definitions: It can be used for finding the positions of the Moon, Sun, and planets without arithmetic operations, using a geometrical model to represent the position of a given celestial body.

Source: https://en.wikipedia.org/wiki/Equatorium""" .


###  http://visualdataweb.org/SpaceScience/Evolutionary_Endpoints
:Evolutionary_Endpoints rdf:type owl:Class ;
                        rdfs:subClassOf :Star ;
                        rdfs:comment """Definition: The points at which the life cycle of a star ends. 

Justification: Classification based on their masses or the Chandrasekhar limit.""" .


###  http://visualdataweb.org/SpaceScience/Extra_Solar
:Extra_Solar rdf:type owl:Class ;
             rdfs:subClassOf :Astronomical_Phenomena ;
             rdfs:comment """Definition: Phenomena occurring outside our solar system.

Justification: Classification based on astronomical objects involved.""" .


###  http://visualdataweb.org/SpaceScience/Extragalactic_Cosmic_Rays
:Extragalactic_Cosmic_Rays rdf:type owl:Class ;
                           rdfs:subClassOf :G_Energetic_Particles ;
                           owl:disjointWith :Galactic_Wind ;
                           rdfs:comment """Definition: Extragalactic cosmic rays (ECRs) are ultra-high energy particles,
thought to originate in active galactic nuclei, in star-forming galaxies,
and from sources still unknown.""" .


###  http://visualdataweb.org/SpaceScience/G_Binary
:G_Binary rdf:type owl:Class ;
          rdfs:subClassOf :Galaxy_Systems ;
          rdfs:comment "Definition: A binary galaxy, sometimes called a double galaxy, consists of two galaxies either orbiting one another in bound orbits or involved in close encounters." .


###  http://visualdataweb.org/SpaceScience/G_Cluster
:G_Cluster rdf:type owl:Class ;
           rdfs:subClassOf :Galaxy_Systems ;
           rdfs:comment """Definition: A cluster of galaxies is a gravitationally bound aggregation of galaxies
intermediate in size between a Galaxy Group (G 21) and a
Supercluster (G 23). Galaxy clusters are given the name of the constellation
in which they are found, and typically contain between
50 and 1,000 galaxies, though some may contain up to 2,000 galaxies.

Justification: Classification based on structure of its core.""" .


###  http://visualdataweb.org/SpaceScience/G_Dust
:G_Dust rdf:type owl:Class ;
        rdfs:subClassOf :Intergalactic_Medium ;
        rdfs:comment """Definition: Intergalactic dust
consists of small particles found between galaxies, believed to originate
in dying stars and driven out of galaxies, along with gas, by
stellar and galactic winds (S 29 and G 17) as well as radiation pressure.""" .


###  http://visualdataweb.org/SpaceScience/G_Energetic_Particles
:G_Energetic_Particles rdf:type owl:Class ;
                       rdfs:subClassOf :Intergalactic_Medium ;
                       rdfs:comment """Definition: Definition: In the physical sciences, a particle (or corpuscule in older texts) is a small localized object to which can be ascribed several physical or chemical properties, such as volume, density, or mass.

Source: https://en.wikipedia.org/wiki/Particle#:~:text=In%20the%20physical%20sciences%2C%20a,volume%2C%20density%2C%20or%20mass.

Justification: Classification based on origin of the Particles""" .


###  http://visualdataweb.org/SpaceScience/G_Gas
:G_Gas rdf:type owl:Class ;
       rdfs:subClassOf :Intergalactic_Medium ;
       rdfs:comment """Definition: Intergalactic gas is a hot, highly rarefied
plasma consisting primarily of ionized hydrogen, along with
traces of other elements such as helium and oxygen.

Justification: Classification based on the temperature of the Gas.""" .


###  http://visualdataweb.org/SpaceScience/G_Group
:G_Group rdf:type owl:Class ;
         rdfs:subClassOf :Galaxy_Systems ;
         rdfs:comment """Definition: Beyond binary galaxies (G 19), a galaxy
group has usually been considered a collection of between
three and 50 gravitationally bound galaxies spanning less than 10
million light years.""" .


###  http://visualdataweb.org/SpaceScience/G_Interacting
:G_Interacting rdf:type owl:Class ;
               rdfs:subClassOf :Galaxy_Systems ;
               rdfs:comment """Definition: Interacting galaxies are two or more galaxies substantially disturbing
each other due to mutual gravitational attraction. Interactions
range from minor disturbances, such as a disruption of spiral arms,
to full-on galaxy collisions.

Justification: Classification based on the stage of interaction the galaxies currently are.""" .


###  http://visualdataweb.org/SpaceScience/G_Supercluster
:G_Supercluster rdf:type owl:Class ;
                rdfs:subClassOf :Galaxy_Systems ;
                rdfs:comment """Definition: Through the relentless reach of gravitation, clusters of galaxies
may form superclusters spanning a hundred million light years or
more, ten times more extensive than clusters (G 22). Like clusters,
superclusters are distinguished by their gravitational interaction
at these much larger scales, which tends to pull them together,
overcoming some of the Hubble flow due to the expansion of the
universe.""" .


###  http://visualdataweb.org/SpaceScience/Galactic_Cosmic_Rays
:Galactic_Cosmic_Rays rdf:type owl:Class ;
                      rdfs:subClassOf :S_Energetic_Particles ;
                      owl:disjointWith :Stellar_Wind ;
                      rdfs:comment """Definition: Galactic cosmic rays (GCRs) are energetic particles with energies
ranging from about 100 MeV to ten GeV (108 to 1010 electron volts)
and more, corresponding respectively to 43% and 99.6% of the
speed of light for protons.
Galactic cosmic rays are believed to originate within our own Galaxy in the expanding shockwaves of supernovae explosions

Source: Classifying the Cosmos (Book)""" .


###  http://visualdataweb.org/SpaceScience/Galactic_Halo
:Galactic_Halo rdf:type owl:Class ;
               rdfs:subClassOf :Circumgalactic ;
               rdfs:comment """Definition: A halo is a slightly flattened spherical population of stars, globular
clusters (S 35), and diffuse ionized gas surrounding disk galaxies,
including spirals (G 4) and lenticulars (G 3), as well as some types
of massive elliptical galaxies""" .


###  http://visualdataweb.org/SpaceScience/Galactic_Jet
:Galactic_Jet rdf:type owl:Class ;
              rdfs:subClassOf :Circumgalactic ;
              rdfs:comment """Definition: Galactic jets are energetic emissions of matter associated with
supermassive black holes in the nuclei of active galaxies.""" .


###  http://visualdataweb.org/SpaceScience/Galactic_Ring
:Galactic_Ring rdf:type owl:Class ;
               rdfs:subClassOf :Circumgalactic ;
               rdfs:comment """Definition: Just as satellites orbit planets and planets orbit stars, so do galaxies
have their own satellites and circumgalactic material orbiting them, notably in the form of smaller galaxies or their shredded debris known as rings or stellar streams.
Like planetary rings and stellar disks and shells, galaxies show a variety of ring structures associated with the merger of galaxies and the formation of galactic halos""" .


###  http://visualdataweb.org/SpaceScience/Galactic_Wind
:Galactic_Wind rdf:type owl:Class ;
               rdfs:subClassOf :G_Energetic_Particles ;
               rdfs:comment """Definition: Galactic winds are streams of charged particles, gas and dust that
blow off galaxies, analogous to solar wind (P 16) and stellar wind
(S 29), creating filaments and bubbles of multi-million-degree gas
clouds that may extend tens of thousands of light years from the
galaxies themselves.
Galactic winds are believed to originate with massive
stars, supernovae, and the black holes of active galactic nuclei.""" .


###  http://visualdataweb.org/SpaceScience/Galaxy
:Galaxy rdf:type owl:Class ;
        rdfs:subClassOf :Kingdom_of_Galaxies ;
        rdfs:comment """Definition: A galaxy is a gravitationally bound system of stars, stellar remnants, interstellar gas, dust, and dark matter.

Source: https://en.wikipedia.org/wiki/Galaxy

Justification: Classfication based on the position of supermassive black hole in the galaxy""" .


###  http://visualdataweb.org/SpaceScience/Galaxy_Merger
:Galaxy_Merger rdf:type owl:Class ;
               rdfs:subClassOf :Involving_Galaxies ;
               rdfs:comment "Definition: Galaxy mergers can occur when two (or more) galaxies collide. They are the most violent type of galaxy interaction." .


###  http://visualdataweb.org/SpaceScience/Galaxy_Systems
:Galaxy_Systems rdf:type owl:Class ;
                rdfs:subClassOf :Kingdom_of_Galaxies ;
                rdfs:comment """Definition: Definition: A system is a group of interacting or interrelated elements that act according to a set of rules to form a unified whole.

Source: https://en.wikipedia.org/wiki/System

Justification: Classification based on the amount of galaxies involved and gravitational interaction among  the galaxies.""" .


###  http://visualdataweb.org/SpaceScience/Gas
:Gas rdf:type owl:Class ;
     rdfs:subClassOf :Interplanetary_Medium ;
     rdfs:comment """Definition: Interplanetary gas is a rarefied neutral gas flowing through
the Solar System at a speed of about 25 km/sec.
Interplanetary gas is thus a rarefied interstellar wind that differs
from the much denser solar wind, which is composed of energetic
charged particles emanating from the Sun at very high speeds.

Source: Classifying the Cosmos (Book)""" .


###  http://visualdataweb.org/SpaceScience/Gas_Giant
:Gas_Giant rdf:type owl:Class ;
           rdfs:subClassOf :Planet ;
           rdfs:comment """Definition: a gas giant planet is one whose main constituents are hydrogen and helium, and whose gaseous/liquid component is larger than the core, which
may be rocky or metallic.

Source: Classifying the cosmos (Book)""" .


###  http://visualdataweb.org/SpaceScience/Giant
:Giant rdf:type owl:Class ;
       rdfs:subClassOf :Post-Main_Sequence ;
       rdfs:comment """Definition: Giant stars are those stars that have ceased their core hydrogen
burning and left the main sequence on the HR diagram. Giants have masses up to five times, and luminosities hundreds of times, that of the Sun.

Source: Classifying the Cosmos (Book)""" .


###  http://visualdataweb.org/SpaceScience/Globular_Cluster
:Globular_Cluster rdf:type owl:Class ;
                  rdfs:subClassOf :Star_Systems ;
                  rdfs:comment """Definition: If open stars clusters are analogous to young towns, globular clusters
are its large cities. Named for their spherical appearance, “globulars” are concentrations of tens of thousands to millions of stars.""" .


###  http://visualdataweb.org/SpaceScience/Herbig-Haro_Object
:Herbig-Haro_Object rdf:type owl:Class ;
                    rdfs:subClassOf :Circumstellar ;
                    rdfs:comment """Definition: Herbig-Haro Objects are small bright patches of nebulosity formed
when the gas from a stellar jet (S 20) collides with gas in the interstellar
medium.

Source: Classifying the Cosmos (Book)""" .


###  http://visualdataweb.org/SpaceScience/High_Luminosity
:High_Luminosity rdf:type owl:Class ;
                 rdfs:subClassOf :Elliptical ;
                 owl:disjointWith :Low_Luminosity ;
                 rdfs:comment """Definition: Has comparetively higher luminosity

Justification: Classification based on presence of nuclear core.""" .


###  http://visualdataweb.org/SpaceScience/High_Surface_Brightness
:High_Surface_Brightness rdf:type owl:Class ;
                         rdfs:subClassOf :Low_Luminosity ;
                         rdfs:comment "Definition: Has higher surface brightness." .


###  http://visualdataweb.org/SpaceScience/Hot_Ionized_Cloud
:Hot_Ionized_Cloud rdf:type owl:Class ;
                   rdfs:subClassOf :S_Gas ;
                   rdfs:comment """Definition: Unlike H I regions consisting of cold neutral hydrogen (S 23), H
II regions are clouds of hot ionized hydrogen where the electrons
have become separated from their parent protons through the
absorption of ultraviolet photons from a nearby star.

Source: Classifying the Cosmos (Book)""" .


###  http://visualdataweb.org/SpaceScience/Hypergiant
:Hypergiant rdf:type owl:Class ;
            rdfs:subClassOf :Post-Main_Sequence ;
            rdfs:comment """Definition: A hypergiant (luminosity class 0 or Ia+) is a very rare type of star that has an extremely high luminosity, mass, size and mass loss because of its extreme stellar winds.

Source: https://en.wikipedia.org/wiki/Hypergiant""" .


###  http://visualdataweb.org/SpaceScience/Ice_Giant
:Ice_Giant rdf:type owl:Class ;
           rdfs:subClassOf :Planet ;
           rdfs:comment """Definition:An ice giant is a planet whose outer constituents are made of
elements heavier than hydrogen and helium—probably water,
ammonia, and methane—and whose dense cores may dominate
the gaseous component.

Source: Classifying the cosmos (Book)""" .


###  http://visualdataweb.org/SpaceScience/Interferometer
:Interferometer rdf:type owl:Class ;
                rdfs:subClassOf :Recording ;
                rdfs:comment "Definition: The interferometer is a type of astronomical instrument that can help determine the size of a celestial object. These instruments collect data on the interference pattern of the phenomenon." .


###  http://visualdataweb.org/SpaceScience/Intergalactic_Medium
:Intergalactic_Medium rdf:type owl:Class ;
                      rdfs:subClassOf :Kingdom_of_Galaxies ;
                      rdfs:comment """Definition: The space between galaxies is emptier than the best vacuum we can make in the lab. However, when viewed from a grand astronomical perspective, the small amount of matter adds up to make the “intergalactic medium”. This tenuous gas is extremely hot, and contains matter swept out of galaxies by star formation, black holes, interactions between galaxies, and possibly other phenomena which we have yet to discover.

Source: https://www.cfa.harvard.edu/research/topic/intergalactic-medium

Justification: Classification based on the type of matter.""" .


###  http://visualdataweb.org/SpaceScience/Intermediate
:Intermediate rdf:type owl:Class ;
              rdfs:subClassOf :G_Interacting .


###  http://visualdataweb.org/SpaceScience/Intermediate_Black_Hole
:Intermediate_Black_Hole rdf:type owl:Class ;
                         rdfs:subClassOf :Black_Hole ;
                         rdfs:comment """Definition: Few thousand solar masses, found at the centers
of globular clusters, S 35

Source: Classifying the Cosmos (Book)""" .


###  http://visualdataweb.org/SpaceScience/Interplanetary_Medium
:Interplanetary_Medium rdf:type owl:Class ;
                       rdfs:subClassOf :Kingdom_of_Planets ;
                       rdfs:comment """Definition: The interplanetary medium (IPM) or interplanetary space consists of the mass and energy which fills the Solar System, and through which all the larger Solar System bodies, such as planets, dwarf planets, asteroids, and comets, move. The IPM stops at the heliopause, outside of which the interstellar medium begins.

Source:https://en.wikipedia.org/wiki/Interplanetary_medium#:~:text=The%20interplanetary%20medium%20(IPM)%20or,which%20the%20interstellar%20medium%20begins.

Justification: Classification based on the type of the matter.""" .


###  http://visualdataweb.org/SpaceScience/Interstellar_Medium
:Interstellar_Medium rdf:type owl:Class ;
                     rdfs:subClassOf :Kingdom_of_Stars ;
                     rdfs:comment """Definition: In astronomy, the interstellar medium is the matter and radiation that exist in the space between the star systems in a galaxy.

Source: https://en.wikipedia.org/wiki/Interstellar_medium#:~:text=In%20astronomy%2C%20the%20interstellar%20medium,into%20the%20surrounding%20intergalactic%20space.

Justification: Classification based on the type of matter.""" .


###  http://visualdataweb.org/SpaceScience/Involving_Galaxies
:Involving_Galaxies rdf:type owl:Class ;
                    rdfs:subClassOf :Extra_Solar ;
                    rdfs:comment """Definition: Astronomical phenomenas outside our solar system involving Galaxies.

Justification: Classificaiton based on the manner in which the event occur""" .


###  http://visualdataweb.org/SpaceScience/Involving_Stars
:Involving_Stars rdf:type owl:Class ;
                 rdfs:subClassOf :Extra_Solar ;
                 rdfs:comment """Definition: Astronomical phenomenas outside our solar system involving Stars.

Justification: Classification based on the manner in which the event occurs.""" .


###  http://visualdataweb.org/SpaceScience/Irregular_Cluster
:Irregular_Cluster rdf:type owl:Class ;
                   rdfs:subClassOf :G_Cluster ,
                                   :Normal ;
                   owl:disjointWith :Regular_Cluster ;
                   rdfs:comment "Definition: Irregular clusters have no well-defined center and often include all galaxy types." .


###  http://visualdataweb.org/SpaceScience/Kingdom_of_Galaxies
:Kingdom_of_Galaxies rdf:type owl:Class ;
                     rdfs:subClassOf :Astronomical_Objects ;
                     rdfs:comment """Definition: With the Kingdom of the Galaxies we enter a realm not recognized
until a century ago, when certain “nebulae” thought to be within
our own Galaxy were found to be extremely distant “extragalactic”
systems of stars—galaxies in their own right. This relatively
new Kingdom encompasses both previous Kingdoms, harboring
stars and planets, clustering into systems and hierarchies of systems
more readily than even stellar systems.

Source: Classfiying the Cosmos by Steven J. Dick (Book)

Justification: Classification based on the Galaxy’s origin(Proto-), location (Circum- and Inter-), subsidiary status (Sub-) and tendency to form systems (Systems). Subclasses are delineated by the various manifestations of the gravitational force acting on astronomical objects.""" .


###  http://visualdataweb.org/SpaceScience/Kingdom_of_Planets
:Kingdom_of_Planets rdf:type owl:Class ;
                    rdfs:subClassOf :Astronomical_Objects ;
                    rdfs:comment """Definition: The Kingdom of the Planets is the realm of astronomy most familiar
in popular culture. This largely has to do with the fact that its
objects are closest to our home planet and thus are most easily
observable both from the ground and—uniquely among the Three
Kingdoms—from in situ spacecraft.

Source: Classfiying the Cosmos by Steven J. Dick (Book)

Justification: Classification based on the Planet’s origin(Proto-), location (Circum- and Inter-), subsidiary status (Sub-) and tendency to form systems (Systems).""" .


###  http://visualdataweb.org/SpaceScience/Kingdom_of_Stars
:Kingdom_of_Stars rdf:type owl:Class ;
                  rdfs:subClassOf :Astronomical_Objects ;
                  rdfs:comment """Defintion:With the Kingdom of the Stars we enter a more distant realm,
where gaseous rather than solid objects reign, and with additional
physics from the hydrostatics laws dominating the planets.
Gravity and hydrostatics are still our constant companions, but
here they work their will in different ways.

Source: Classfiying the Cosmos by Steven J. Dick (Book)

Justification: Classification based on the Star’s origin(Proto-), location (Circum- and Inter-), subsidiary status (Sub-) and tendency to form systems (Systems).""" .


###  http://visualdataweb.org/SpaceScience/Kuiper_Belt
:Kuiper_Belt rdf:type owl:Class ;
             rdfs:subClassOf :Trans-Neptunian_Systems ;
             owl:disjointWith :Oort_Cloud ;
             rdfs:comment """Definition: Kuiper belt objects (KBOs) include those trans-Neptunian objects
(P 13) that reside in stable orbits around the Sun in the space
extending from 30 to approximately 55 astronomical units (AU)
from the Sun, as well as those less dynamically stable objects
known as scattered-disk objects that may extend as far as 2,000
AU.

Source: Classifying the Cosmos (Book)

Justification: Classification based on their orbital characteristics.""" .


###  http://visualdataweb.org/SpaceScience/Lenticular
:Lenticular rdf:type owl:Class ;
            rdfs:subClassOf :Normal ;
            rdfs:comment """Definition: Lenticular galaxies are gravitationally bound conglomerations of
stars with a rotating disk and a central bulge, but no spiral arms or
dust lanes. In many ways they are intermediate in nature between
elliptical and spiral galaxies, devoid of gas and dust like ellipticals
but with some structure like spirals.""" .


###  http://visualdataweb.org/SpaceScience/Libration
:Libration rdf:type owl:Class ;
           rdfs:subClassOf :Single_Objects ;
           rdfs:comment "Definition: libration is the wagging or wavering of the Moon perceived by Earth-bound observers and caused by changes in their perspective. It permits an observer to see slightly different hemispheres of the surface at different times." ;
           rdfs:label "Libration"@en .


###  http://visualdataweb.org/SpaceScience/Low_Luminosity
:Low_Luminosity rdf:type owl:Class ;
                rdfs:subClassOf :Elliptical ;
                rdfs:comment """Definition: Has lower luminosity

Justification: Classification based on surface brightness.""" .


###  http://visualdataweb.org/SpaceScience/Low_Surface_Brightness
:Low_Surface_Brightness rdf:type owl:Class ;
                        rdfs:subClassOf :Low_Luminosity ;
                        rdfs:comment "Definition: Has low surface brightness." .


###  http://visualdataweb.org/SpaceScience/Lunar_Eclipse
:Lunar_Eclipse rdf:type owl:Class ;
               rdfs:subClassOf :Ecplise ;
               rdfs:comment "Definition: Solar eclipses can only occur during a New Moon when the Moon moves between Earth and the Sun, and the three celestial bodies form a straight line: Earth–Moon–Sun." ;
               rdfs:label "Lunar Eclipse"@en .


###  http://visualdataweb.org/SpaceScience/Lyman_alpha_blobs
:Lyman_alpha_blobs rdf:type owl:Class ;
                   rdfs:subClassOf :G_Gas ;
                   owl:disjointWith :Warm_Hot_IGM ;
                   rdfs:comment """Definition: Lyman alpha blobs are large concentrations of hydrogen gas in the
intergalactic medium (IGM), spanning several hundred thousand
light years and emitting light at the “Lyman alpha” wavelength
produced when electrons recombine with ionized hydrogen.""" .


###  http://visualdataweb.org/SpaceScience/Main_Sequence
:Main_Sequence rdf:type owl:Class ;
               rdfs:subClassOf :Star ;
               rdfs:comment """Definition: A main sequence star is any star that has a hot, dense core which fuses hydrogen into helium to produce energy. 

Source: https://study.com/academy/lesson/main-sequence-star-definition-facts-quiz.html#:~:text=Lesson%20Summary-,What%20is%20a%20Main%20Sequence%20Star%3F,Tau%20Ceti%20and%20the%20Sun.

Justification: Classification based on the luminosities of the star.""" .


###  http://visualdataweb.org/SpaceScience/Meteor_Shower
:Meteor_Shower rdf:type owl:Class ;
               rdfs:subClassOf :Single_Objects ;
               rdfs:comment """Definition: A meteor shower is a celestial event in which a number of meteors are observed to radiate, or originate, from one point in the night sky called Radiant. These meteors are caused by streams of cosmic debris called meteoroids entering Earth's atmosphere at extremely high speeds on parallel trajectories.

Source: https://www.amsmeteors.org/meteor-showers/meteor-shower-calendar/#:~:text=A%20meteor%20shower%20is%20a,high%20speeds%20on%20parallel%20trajectories.""" .


###  http://visualdataweb.org/SpaceScience/Meteoroid
:Meteoroid rdf:type owl:Class ;
           rdfs:subClassOf :Subplanetary ;
           rdfs:comment """Definition: Meteoroids are debris particles ranging in size from grains of sand
to boulders traveling in solar orbits that may occasionally intersect
the orbit of the Earth

Source: Classifying the cosmos (Book)""" .


###  http://visualdataweb.org/SpaceScience/Meteroid_streams
:Meteroid_streams rdf:type owl:Class ;
                  rdfs:subClassOf :Systems ;
                  rdfs:comment """Definition: A meteoroid stream is a collection of meteoroids believed
to be shed from a short-period comet during its perihelion
passage, or from an Earth-crossing asteroid.

Source: Classifying the Cosmos (Book)""" .


###  http://visualdataweb.org/SpaceScience/Mirror_lens
:Mirror_lens rdf:type owl:Class ;
             rdfs:subClassOf :Telescope .


###  http://visualdataweb.org/SpaceScience/Molecular_Cloud
:Molecular_Cloud rdf:type owl:Class ;
                 rdfs:subClassOf :S_Gas ;
                 rdfs:comment """Definition: A molecular cloud is an interstellar gas cloud dense enough to permit
formation of molecules, mostly hydrogen (H2) but also laced
with more complex molecules

Source: Classifying the Cosmos (Book)""" .


###  http://visualdataweb.org/SpaceScience/Multiple_Objects
:Multiple_Objects rdf:type owl:Class ;
                  rdfs:subClassOf :Solar ;
                  rdfs:comment """Definition: Astronomical phenomenas within our solar system involving multiple objects

Justification: Classification based on the manner in which the event occur.""" .


###  http://visualdataweb.org/SpaceScience/Multiple_Star
:Multiple_Star rdf:type owl:Class ;
               rdfs:subClassOf :Star_Systems ;
               rdfs:comment """Definition: Multiple stars are gravitationally bound systems with three or
more stars. Although stars can sometimes appear to be multiple by
virtue of their proximity in the sky, these are not true multiples, in
the same way the apparent double stars are not true binary stars.

Source: Classifying the Cosmos (Book)""" .


###  http://visualdataweb.org/SpaceScience/Neutron_Star
:Neutron_Star rdf:type owl:Class ;
              rdfs:subClassOf :Evolutionary_Endpoints ;
              rdfs:comment """Definition: A neutron star results when a stellar core between about 1.4 and 2 or 3 solar masses, having consumed its nuclear fuel at the end of its life, explodes as a supernova , leaving behind a dense core squeezed so tightly it consists only of neutrons.

Source: Classifying the Cosmos (Book)""" .


###  http://visualdataweb.org/SpaceScience/Normal
:Normal rdf:type owl:Class ;
        rdfs:subClassOf :Galaxy ;
        rdfs:comment """Definition: normal galaxies have a supermassive black hole at their center

Source: https://imagine.gsfc.nasa.gov/science/objects/active_galaxies1.html#:~:text=Most%2C%20if%20not%20all%2C%20normal,and%20form%20into%20a%20disk.

Justification: Classification based on morphology of the galaxy.""" .


###  http://visualdataweb.org/SpaceScience/Nova_Remnant
:Nova_Remnant rdf:type owl:Class ;
              rdfs:subClassOf :Circumstellar ;
              rdfs:comment """Definition: A nova is a close binary star (S 31) usually consisting of a white
dwarf (S 12) and a main sequence normal star, in which hydrogen
from the normal star is accreted onto the white dwarf.
A nova remnant,  still surrounds its parent stars
and is thus a circumstellar object. While it might seem that a nova
and a supernova should both have class status at the same taxon
level, they are in fact two very different phenomena, with a supernova
white dwarf exploding and being destroyed while a nova
white dwarf repeatedly erupts over a period of time.

Source: Classifying the Cosmos (Book)""" .


###  http://visualdataweb.org/SpaceScience/Novae
:Novae rdf:type owl:Class ;
       rdfs:subClassOf :Involving_Stars ;
       rdfs:comment "Definition: A nova (plural novae or novas) is a transient astronomical event that causes the sudden appearance of a bright, apparently \"new\" star that slowly fades over weeks or months." ;
       rdfs:label "Novae"@en ,
                  "Novae"@iri-based .


###  http://visualdataweb.org/SpaceScience/Observational
:Observational rdf:type owl:Class ;
               rdfs:subClassOf :Earth_Instrument ;
               rdfs:comment """Definition: instruments that are used for observation. Observational astronomical instruments can be used to determine the size and structure of a celestial object.

Source: https://www.allthescience.org/what-are-the-different-types-of-astronomical-instruments.htm

Justification: Classification based on the scope of use""" .


###  http://visualdataweb.org/SpaceScience/Oort_Cloud
:Oort_Cloud rdf:type owl:Class ;
            rdfs:subClassOf :Trans-Neptunian_Systems ;
            rdfs:comment """Definition: The Oort cloud, occasionally called the Öpik-Oort cloud, is a
spherical reservoir of trans-Neptunian objects surrounding
the Solar System. If the Kuiper belt is the Solar System’s
“third zone” beyond the terrestrial and gas giants, the Oort cloud
is its fourth zone, and the one containing most of its objects.

Source: Classifying the Cosmos (Book)""" .


###  http://visualdataweb.org/SpaceScience/Open_Cluster
:Open_Cluster rdf:type owl:Class ;
              rdfs:subClassOf :Star_Systems ;
              rdfs:comment """Definition: An open cluster (also known as a galactic cluster) is a group of hundreds to thousands of stars formed in the same molecular cloud
(S 25) and still loosely bound gravitationally.""" .


###  http://visualdataweb.org/SpaceScience/Outer_Space
:Outer_Space rdf:type owl:Class ;
             rdfs:subClassOf :Astronomical_Instruments ;
             rdfs:comment """Definition: Artifical Objects in outer space

Justification: Classification based on the orbital state, especially  if it is a controlled or uncontrolled orbit

Note:
Prefixes in this classificaiton are the Initial letter of its superclasses.""" .


###  http://visualdataweb.org/SpaceScience/Photometric
:Photometric rdf:type owl:Class ;
             rdfs:subClassOf :Binary ;
             rdfs:comment """Definition: distinguished by light variations

Source: Classifying the Cosmos (Book)""" .


###  http://visualdataweb.org/SpaceScience/Planet
:Planet rdf:type owl:Class ;
        rdfs:subClassOf :Kingdom_of_Planets ;
        rdfs:comment """Definition: A planet is a large, rounded astronomical body that is neither a star nor its remnant.

Source: https://en.wikipedia.org/wiki/Planet

Justification: Classification based on its constituents""" .


###  http://visualdataweb.org/SpaceScience/Planet_Radiation_Belt
:Planet_Radiation_Belt rdf:type owl:Class ;
                       rdfs:subClassOf :Circumplanetary ;
                       rdfs:comment """Definition: A planetary radiation belt is a reservoir of energetic charged particles surrounding a planet and trapped in the magnetosphere created by the planet’s internally generated magnetic field.

Source: Classifying the cosmos (Book)""" .


###  http://visualdataweb.org/SpaceScience/Planetary_Nebula
:Planetary_Nebula rdf:type owl:Class ;
                  rdfs:subClassOf :Circumstellar ;
                  rdfs:comment """Definition: A planetary nebula represents one of the steps on the way to the
evolutionary endpoint of a low-mass star like the Sun. It occurs
when the dying star, having expanded to a red giant, ejects its outer
envelope.

Source: Classifying the Cosmos (Book)""" .


###  http://visualdataweb.org/SpaceScience/Planetary_Ring
:Planetary_Ring rdf:type owl:Class ;
                rdfs:subClassOf :Circumplanetary ;
                rdfs:comment """Defintion: Planetary rings consist of particle- to house-sized objects orbiting
a planet, forming one of the great spectacles of the Solar System.

Source: Classifying the cosmos (Book)""" .


###  http://visualdataweb.org/SpaceScience/Planetary_Systems
:Planetary_Systems rdf:type owl:Class ;
                   rdfs:subClassOf :Systems ;
                   rdfs:comment """Definition: A system composed of planets. Because of their mechanism of formation, planets tend to exist in systems, each bound to its central star. A planetary system consists not only of the planets themselves but also everything associated with them.

Source: Classifying the Cosmos (Book)""" .


###  http://visualdataweb.org/SpaceScience/Plantetary_Satellite
:Plantetary_Satellite rdf:type owl:Class ;
                      rdfs:subClassOf :Circumplanetary ;
                      rdfs:comment """Definition: The term “natural satellite” most commonly refers to a body such
as the Moon orbiting a planet, but it also applies to bodies orbiting
minor planets, dwarf planets, and Kuiper belt objects.

Source: Classifying the cosmos (Book)""" .


###  http://visualdataweb.org/SpaceScience/Population
:Population rdf:type owl:Class ;
            rdfs:subClassOf :Star_Systems ;
            rdfs:comment """Definition: Like the citizens of countries, stars may be divided into broad
“populations” based on location. Unlike citizens, however, stellar
populations are often highly correlated with age and chemical
composition.

Justification: Classification based on age of the stars.""" .


###  http://visualdataweb.org/SpaceScience/Population_I
:Population_I rdf:type owl:Class ;
              rdfs:subClassOf :Population ;
              rdfs:comment "Definition: Population I stars are the youngest" .


###  http://visualdataweb.org/SpaceScience/Population_II
:Population_II rdf:type owl:Class ;
               rdfs:subClassOf :Population ;
               rdfs:comment "Definition: Population II are intermediate in age" .


###  http://visualdataweb.org/SpaceScience/Population_III
:Population_III rdf:type owl:Class ;
                rdfs:subClassOf :Population ;
                rdfs:comment "Definition: Population III are the oldest" .


###  http://visualdataweb.org/SpaceScience/Post-Main_Sequence
:Post-Main_Sequence rdf:type owl:Class ;
                    rdfs:subClassOf :Star ;
                    rdfs:comment """Definition: A post-main-sequence star is a star that has been through a main-sequence phase (the primary, lengthy phase of hydrogen-burning fusion in the center, i.e., it is beyond TAMS, terminal-age main sequence) and is proceeding through additional phases, sometimes including fusion of various elements.

Source: http://astro.vaporia.com/start/postmainsequencestar.html#:~:text=A%20post%2Dmain%2Dsequence%20star,including%20fusion%20of%20various%20elements.

Justification:Classificaiton based on the absolute magnitude and size of the stars. 
Absolute magnitude is defined as the brightness of stars if they were all
observed from the same distance of 10 parsecs (32.6 light years).""" .


###  http://visualdataweb.org/SpaceScience/Pre-Main_Sequence
:Pre-Main_Sequence rdf:type owl:Class ;
                   rdfs:subClassOf :Star ;
                   rdfs:comment """Definition: A pre-main-sequence star (also known as a PMS star and PMS object) is a star in the stage when it has not yet reached the main sequence. 

Source: https://en.wikipedia.org/wiki/Pre-main-sequence_star

Justification: Classification based on the mass.""" .


###  http://visualdataweb.org/SpaceScience/Protogalactic
:Protogalactic rdf:type owl:Class ;
               rdfs:subClassOf :Kingdom_of_Galaxies ;
               rdfs:comment "Definition: Like protoplanets (P 1) and protostars (S 1), galaxies must be born." .


###  http://visualdataweb.org/SpaceScience/Protogalaxy
:Protogalaxy rdf:type owl:Class ;
             rdfs:subClassOf :Protogalactic ;
             rdfs:comment """Definition: The earliest galaxies existed at least 500 million years after
the Big Bang, so in a technical sense these were the first protogalaxies.
The definition of a protogalaxy is somewhat nebulous, so to speak.
Given the uncertainties, an operational definition might be that a protogalaxy ends and a galaxy begins when stars light up the galaxy, and the wind from star formation and supernovae, as well as black hole accretion, exceeds the gravity
of the host galaxy.""" .


###  http://visualdataweb.org/SpaceScience/Protoplanetary
:Protoplanetary rdf:type owl:Class ;
                rdfs:subClassOf :Kingdom_of_Planets ;
                rdfs:comment """Definition: All things must be born, and for planets birth begins with a protoplanetary disk, a circumstellar disk of gas and dust that originates
during star formation, when a protostar condenses out of a
molecular cloud.

Source: Classifying the Cosmos - How we can make sense of the celestial landscape

Justification: Hubble Space Telescope observations first proved the existence
of protoplanetary objects in the form of proplyds. Hence only one subclass.""" .


###  http://visualdataweb.org/SpaceScience/Protostar
:Protostar rdf:type owl:Class ;
           rdfs:subClassOf :Protostellar ;
           rdfs:comment """Definition: A protostar, sometimes called an embryonic star, is a
molecular cloud (S 25) undergoing gravitational contraction and
accretion of gas and dust prior to initiating fusion reactions.""" .


###  http://visualdataweb.org/SpaceScience/Protostellar
:Protostellar rdf:type owl:Class ;
              rdfs:subClassOf :Kingdom_of_Stars ;
              rdfs:comment """Definition: Like planets, stars are born, but they do so in considerably more
spectacular fashion and at rates highly dependent on their environment.""" .


###  http://visualdataweb.org/SpaceScience/Pulsar_Planet
:Pulsar_Planet rdf:type owl:Class ;
               rdfs:subClassOf :Planet ;
               rdfs:comment """Definition: Their composition is likely very different from other types of planets, since they must be built from stellar rubble (iron, nitrogen, and other heavy elements) that survived a supernova explosion ending in a neutron
star.

Source: Classifying the cosmos (Book)""" .


###  http://visualdataweb.org/SpaceScience/Quasar
:Quasar rdf:type owl:Class ;
        rdfs:subClassOf :Active ;
        rdfs:comment "Definitions: Quasars are now known to be the cores of extremely distant active galaxies, the most luminous of all classes of active galaxies discovered before or since, including Seyferts (G 6), radio galaxies (G 7), and blazars (G 9)." .


###  http://visualdataweb.org/SpaceScience/Radio_Galaxy
:Radio_Galaxy rdf:type owl:Class ;
              rdfs:subClassOf :Active ;
              rdfs:comment """Definition: Unlike Seyferts with their intense optical emission, radio
galaxies exhibit intense radio emission. They are almost always
large elliptical galaxies, by contrast to the Seyfert class, which are
normally spirals.""" .


###  http://visualdataweb.org/SpaceScience/Recording
:Recording rdf:type owl:Class ;
           rdfs:subClassOf :Earth_Instrument ;
           rdfs:comment """Definition: Instruments used to record data

Justification: Classification based on scope of use""" .


###  http://visualdataweb.org/SpaceScience/Reflection_Nebulae
:Reflection_Nebulae rdf:type owl:Class ;
                    rdfs:subClassOf :S_Dust ;
                    rdfs:comment """Definition: Reflection nebulae are clouds of dust that do not shine by their
own light, but by light reflected from a nearby star

Source: Classifying the Cosmos (Book)""" .


###  http://visualdataweb.org/SpaceScience/Reflective
:Reflective rdf:type owl:Class ;
            rdfs:subClassOf :Telescope ;
            rdfs:comment "Definition: A reflecting telescope (also called a reflector) is a telescope that uses a single or a combination of curved mirrors that reflect light and form an image." .


###  http://visualdataweb.org/SpaceScience/Refracting
:Refracting rdf:type owl:Class ;
            rdfs:subClassOf :Telescope ;
            rdfs:comment "Definition: A refracting telescope (also called a refractor) is a type of optical telescope that uses a lens as its objective to form an image (also referred to a dioptric telescope)." .


###  http://visualdataweb.org/SpaceScience/Regular_Cluster
:Regular_Cluster rdf:type owl:Class ;
                 rdfs:subClassOf :G_Cluster ;
                 rdfs:comment "Definition: Regular clusters have a spherical structure and concentrated core and appear to be populated mainly by elliptical galaxies" .


###  http://visualdataweb.org/SpaceScience/Resonant_KBOs
:Resonant_KBOs rdf:type owl:Class ;
               rdfs:subClassOf :Kuiper_Belt ;
               rdfs:comment """Definition: Trapped in 2:3 resonance with Neptune (2 orbits
for every 3 of Neptune), have semi-major axes at about 39.4
AUs.

Source: Classifying the Cosmos (Book)""" .


###  http://visualdataweb.org/SpaceScience/S_Dust
:S_Dust rdf:type owl:Class ;
        rdfs:subClassOf :Interstellar_Medium ;
        rdfs:comment """Definition: Dust is made of fine particles of solid matter.

Source: https://en.wikipedia.org/wiki/Dust

Justification: Classification based on their interaction with light.""" .


###  http://visualdataweb.org/SpaceScience/S_Energetic_Particles
:S_Energetic_Particles rdf:type owl:Class ;
                       rdfs:subClassOf :Interstellar_Medium ;
                       rdfs:comment """Definition: In the physical sciences, a particle (or corpuscule in older texts) is a small localized object to which can be ascribed several physical or chemical properties, such as volume, density, or mass.

Source: https://en.wikipedia.org/wiki/Particle#:~:text=In%20the%20physical%20sciences%2C%20a,volume%2C%20density%2C%20or%20mass.

Justification: Classification based on where they originate from.""" .


###  http://visualdataweb.org/SpaceScience/S_Gas
:S_Gas rdf:type owl:Class ;
       rdfs:subClassOf :Interstellar_Medium ;
       rdfs:comment """Definition: a fluid (such as air) that has neither independent shape nor volume but tends to expand indefinitely.

Source: Classifying the Cosmos (Book)

Justification: Classification based on the constituents of gas.""" .


###  http://visualdataweb.org/SpaceScience/Scattered_KBOs
:Scattered_KBOs rdf:type owl:Class ;
                rdfs:subClassOf :Kuiper_Belt ;
                rdfs:comment """Definition: with large eccentricities and perihelia near 35
AU, are thought to originate from Neptune scattering.

Source: Classifying the Cosmos (Book)""" .


###  http://visualdataweb.org/SpaceScience/Seyfert
:Seyfert rdf:type owl:Class ;
         rdfs:subClassOf :Active ;
         rdfs:comment """Definition: Astronomer Carl Keenan Seyfert (1911–1960) defined as a
class what came to be called “Seyferts” in 1943, based on a galaxy’s
bright optical nuclei, or more specifically on “high excitation
nuclear emission lines superposed on a normal G-type spectrum,”
that is to say, superimposed on a solar-type spectrum.

Justification: Classification based on the strengths and widths of their emission lines.""" .


###  http://visualdataweb.org/SpaceScience/Shell
:Shell rdf:type owl:Class ;
       rdfs:subClassOf :Circumstellar ;
       rdfs:comment """Definition: In addition to circumstellar proplyds and debris disks,
material may exist around a star totally unrelated to planetary formation.
Whereas proplyds by definition surround young stars, and
debris disks such as our own Kuiper belt may linger well past
stellar middle age, circumstellar shells (also called circumstellar
envelopes) are related to mass loss late in stellar evolution, via
stellar winds.

Source: Classifying the Cosmos (Book)""" .


###  http://visualdataweb.org/SpaceScience/Single_Objects
:Single_Objects rdf:type owl:Class ;
                rdfs:subClassOf :Solar ;
                rdfs:comment """Definition: Astronomical phenomenas within our solar system involving a single object.

Justifiction: Classification based on the objects involved.""" .


###  http://visualdataweb.org/SpaceScience/Small_Bodies_of_Solar_System
:Small_Bodies_of_Solar_System rdf:type owl:Class ;
                              rdfs:subClassOf :Subplanetary ;
                              rdfs:comment """Definition: Other smaller bodies in the Solar System

Justification: Classification based on the size of the object in comparison to each other.""" .


###  http://visualdataweb.org/SpaceScience/Solar
:Solar rdf:type owl:Class ;
       rdfs:subClassOf :Astronomical_Phenomena ;
       rdfs:comment """Definition: Phenomena that occur within the Solar System.

Justification: Classification based on the number of objects involved in the event""" .


###  http://visualdataweb.org/SpaceScience/Solar_Eclipse
:Solar_Eclipse rdf:type owl:Class ;
               rdfs:subClassOf :Ecplise ;
               rdfs:comment "Definition: A lunar eclipse occurs when Earth comes between the Sun and the Moon and blocks the Sun's rays from directly reaching the Moon." ;
               rdfs:label "Solar Eclipse"@en .


###  http://visualdataweb.org/SpaceScience/Solar_Storm
:Solar_Storm rdf:type owl:Class ;
             rdfs:subClassOf :Single_Objects ;
             rdfs:comment "Definition: A solar storm is a disturbance on the Sun, which can emanate outward across the heliosphere, affecting the entire Solar System, including Earth and its magnetosphere, and is the cause of space weather in the short-term with long-term patterns comprising space climate." .


###  http://visualdataweb.org/SpaceScience/Solar_Wind
:Solar_Wind rdf:type owl:Class ;
            rdfs:subClassOf :Energetic_Particles ;
            rdfs:comment """Definition: The Sun sends matter as well as light into space. This
“solar wind” consists of a stream of charged particles, primarily
electrons and protons, ejected from the Sun at speeds of 200 to 600
miles per second, about a million miles per hour.

Source: Classifying the Cosmos (Book)""" .


###  http://visualdataweb.org/SpaceScience/Spectrograph
:Spectrograph rdf:type owl:Class ;
              rdfs:subClassOf :Observational ;
              rdfs:comment "Definition: A vital instrument of observational astronomy is the spectrograph. The absorption of specific wavelengths of light by elements allows specific properties of distant bodies to be observed." .


###  http://visualdataweb.org/SpaceScience/Spectroscopic
:Spectroscopic rdf:type owl:Class ;
               rdfs:subClassOf :Binary ;
               rdfs:comment """Definition: distinguished by spectral line shifts due to the stars’ mutual motions

Source: Classifying the Cosmos (Book)""" .


###  http://visualdataweb.org/SpaceScience/Spiral
:Spiral rdf:type owl:Class ;
        rdfs:subClassOf :Normal ;
        rdfs:comment """Definitions: Spiral galaxies are gravitationally bound conglomerations of stars
characterized by complex structure, including flat disks, central
bulges, and spiral arms wound with various degrees of tightness.
The spiral arms are active regions of star formation.""" .


###  http://visualdataweb.org/SpaceScience/Star
:Star rdf:type owl:Class ;
      rdfs:subClassOf :Kingdom_of_Stars ;
      rdfs:comment """Definition: A star is an astronomical object comprising a luminous spheroid of plasma held together by its gravity. The nearest star to Earth is the Sun.

Source: https://en.wikipedia.org/wiki/Star

Justification: Classification based on the difference stages at which the star currently is.""" .


###  http://visualdataweb.org/SpaceScience/Star_Systems
:Star_Systems rdf:type owl:Class ;
              rdfs:subClassOf :Kingdom_of_Stars ;
              rdfs:comment """Definition: A system is a group of interacting or interrelated elements that act according to a set of rules to form a unified whole.

Source: https://en.wikipedia.org/wiki/System

Justification: Classification based on the amount of stars present in the system.""" .


###  http://visualdataweb.org/SpaceScience/Stellar_Black_Hole
:Stellar_Black_Hole rdf:type owl:Class ;
                    rdfs:subClassOf :Black_Hole ;
                    rdfs:comment """Definition: up to tens of  times more massive than the Sun, found, for example, in X-ray binaries, S 31

Source: Classifying the Cosmos (Book)""" .


###  http://visualdataweb.org/SpaceScience/Stellar_Jet
:Stellar_Jet rdf:type owl:Class ;
             rdfs:subClassOf :Circumstellar ;
             rdfs:comment """Definition: Stellar jets are energetic matter and radiation ejected from stars
accreting matter, either at star birth or star death and under certain
other exotic circumstances such as cataclysmic variables and
X-ray binaries.
Jets associated with star formation consist of materials
blasted away from a protostar (S 1), a disk of gas and dust falling
into an embryonic star.

Source: Classifying the Cosmos (Book)""" .


###  http://visualdataweb.org/SpaceScience/Stellar_Occultation
:Stellar_Occultation rdf:type owl:Class ;
                     rdfs:subClassOf :Multiple_Objects ;
                     rdfs:comment """Definition: A stellar occultation occurs when, as viewed from Earth, a bright star passes behind a planetary ring system. These events occur rarely, typically last for hours, and can yield data on the location of ring features that rival spacecraft resolutions.

Source: https://www.sciencedirect.com/topics/earth-and-planetary-sciences/stellar-occultation#:~:text=A%20stellar%20occultation%20occurs%20when,features%20that%20rival%20spacecraft%20resolutions.""" ;
                     rdfs:label "Stellar Occultation"@en ,
                                "Stellar_Occultation"@iri-based .


###  http://visualdataweb.org/SpaceScience/Stellar_Wind
:Stellar_Wind rdf:type owl:Class ;
              rdfs:subClassOf :S_Energetic_Particles ;
              rdfs:comment """Definition: Just as our Sun emits a solar wind consisting of charged
particles from its upper atmosphere, so do a wide variety of other
stars. In fact, all stars are believed to have stellar winds of one
kind or another, including exotic specimens such as white dwarfs.

Source: Classifying the Cosmos (Book)""" .


###  http://visualdataweb.org/SpaceScience/Subdwarf
:Subdwarf rdf:type owl:Class ;
          rdfs:subClassOf :Main_Sequence ;
          rdfs:comment """Definition: Subdwarfs, today more accurately known as “cool subdwarfs,” are
an odd type of star that run about one magnitude below the main
sequence in the Hertzsprung-Russell diagram (Fig. 8.2). They are
usually classed as main sequence stars since they are hydrogen
burning, although near the end of this phase of energy generation.

Source: Classifying the Cosmos (Book)""" .


###  http://visualdataweb.org/SpaceScience/Subgalactic
:Subgalactic rdf:type owl:Class ;
             rdfs:subClassOf :Kingdom_of_Galaxies ;
             rdfs:comment """Definition: The term “subgalactic” is most often used in astronomical literature
in connection with protogalaxies.""" .


###  http://visualdataweb.org/SpaceScience/Subgalactic_Object
:Subgalactic_Object rdf:type owl:Class ;
                    rdfs:subClassOf :Subgalactic ;
                    rdfs:comment """Definition: subgalactic objects are the building blocks of galaxies as part of the “hierarchical clustering” process in the cold dark matter (CDM) theory.
In theory, subgalactic objects could also be failed galaxies, analogous
to the failed stars known as brown dwarfs (S 22) in the substellar
Family (Chapter 10), or they could be remnants of galaxy
formation analogous to dwarf planets (P 9) and the small bodies
of the solar system (P 11, 12, and 13) in the subplanetary Family
(Chapter 4).""" .


###  http://visualdataweb.org/SpaceScience/Subgiant
:Subgiant rdf:type owl:Class ;
          rdfs:subClassOf :Post-Main_Sequence ;
          rdfs:comment """Definition: The subgiants, a class of stars that represents an intermediate
stage in low-mass stellar evolution, between main sequence dwarfs
and giant stars in the HR diagram. 
Subgiants, up to ten times the size of the Sun, have begun
their expansion into red giants, which can grow up to 100 times
the size of the Sun. 

Source: Classifying the Cosmos (Book)""" .


###  http://visualdataweb.org/SpaceScience/Subplanetary
:Subplanetary rdf:type owl:Class ;
              rdfs:subClassOf :Kingdom_of_Planets ;
              rdfs:comment """Definition: Describing bodies smaller than a planet

Source: https://www.definitions.net/definition/subplanetary

Justification: Classification based on the formation of the object and size.""" .


###  http://visualdataweb.org/SpaceScience/Substellar
:Substellar rdf:type owl:Class ;
            rdfs:subClassOf :Kingdom_of_Stars ;
            rdfs:comment """Definition: having less mass than a star : not having the mass required to sustain nuclear fission

Source: https://www.merriam-webster.com/dictionary/substellar

Justification: Classification based on Mass.""" .


###  http://visualdataweb.org/SpaceScience/Supergiant
:Supergiant rdf:type owl:Class ;
            rdfs:subClassOf :Post-Main_Sequence ;
            rdfs:comment """Definition: If giants like Arcturus and Aldebaran seem big, supergiants are
even bigger, with 10 to 70 solar masses, radii up to 1,000 times
the Sun’s, and luminosities hundreds of thousands of times the
Sun’s (Fig. 8.8). They are the result of the evolution of high-mass
stars—those greater than eight solar masses.

Source: Classifying the Cosmos (Book)""" .


###  http://visualdataweb.org/SpaceScience/Supermassive_Black_Hole
:Supermassive_Black_Hole rdf:type owl:Class ;
                         rdfs:subClassOf :Black_Hole ;
                         rdfs:comment """Definition: located at the centers of galaxies (millions to billions of times the mass of the Sun)

Source: Classifying the Cosmos (Book)""" .


###  http://visualdataweb.org/SpaceScience/Systems
:Systems rdf:type owl:Class ;
         rdfs:subClassOf :Kingdom_of_Planets ;
         rdfs:comment """Definition: A system is a group of interacting or interrelated elements that act according to a set of rules to form a unified whole.

Source: https://en.wikipedia.org/wiki/System

Justification: Classification based on the members of the system.""" .


###  http://visualdataweb.org/SpaceScience/Syzygy
:Syzygy rdf:type owl:Class ;
        rdfs:subClassOf :Multiple_Objects ;
        rdfs:comment """Definition: In astronomy, a syzygy is a roughly straight-line configuration of three or more celestial bodies in a gravitational system.

Source: https://en.wikipedia.org/wiki/Syzygy_(astronomy)""" .


###  http://visualdataweb.org/SpaceScience/T-Tauri
:T-Tauri rdf:type owl:Class ;
         rdfs:subClassOf :Pre-Main_Sequence ;
         owl:disjointWith <http://visualdataweb.org/SpaceScience/Herbig_Ae/Herbig_Ae/Herbig_Ae_Be> ;
         rdfs:comment """Definition: T Tauri stars represent a very early stage in the history of a low-mass
star, when the protostar  emerges from the surrounding
molecular cloud, but before sustained core hydrogen burning
on the main sequence of the Hertzsprung-Russell diagram.

Source: Classifying the Cosmos (Book)

Justification: Classification based on presence of Nebulous disk.""" .


###  http://visualdataweb.org/SpaceScience/Telescope
:Telescope rdf:type owl:Class ;
           rdfs:subClassOf :Observational ;
           rdfs:comment """Definition:A telescope is an optical instrument using lenses, curved mirrors, or a combination of both to observe distant objects, or various devices used to observe distant objects by their emission, absorption, or reflection of electromagnetic radiation.
 
Justification: Classification based on how they employ lenses or mirrors in order to capture light""" .


###  http://visualdataweb.org/SpaceScience/Terrestrial
:Terrestrial rdf:type owl:Class ;
             rdfs:subClassOf :Planet ;
             rdfs:comment """Definition: In general, a terrestrial planet is one whose constituents
are rocky and therefore similar to the Earth in composition, by
comparison with the gas giant or ice giant planets

Source: Classifying the cosmos (Book)""" .


###  http://visualdataweb.org/SpaceScience/Trans-Neptunian_Objects
:Trans-Neptunian_Objects rdf:type owl:Class ;
                         rdfs:subClassOf :Small_Bodies_of_Solar_System ;
                         rdfs:comment """Definition: While minor planets and comets mostly orbit the Sun
closer than Neptune, many even larger objects, and with somewhat
different physical characteristics, orbit beyond Neptune.
Such bodies are quite logically termed trans-Neptunian objects, or
TNOs for short, and are likely remnants from the accretion process
in protoplanetary disks during the early Solar System.

Source: Classifying the Cosmos (Book)""" .


###  http://visualdataweb.org/SpaceScience/Trans-Neptunian_Systems
:Trans-Neptunian_Systems rdf:type owl:Class ;
                         rdfs:subClassOf :Systems ;
                         rdfs:comment """Definitions: A system composed of Trans-Neptunian Objects. 

Source: Classifying the Cosmos (Book)

Justification: Classification based on the location of the object wrt the Sun.""" .


###  http://visualdataweb.org/SpaceScience/Transit
:Transit rdf:type owl:Class ;
         rdfs:subClassOf :Multiple_Objects ;
         rdfs:comment "Definition: In astronomy, a transit (or astronomical transit) is a phenomenon when a celestial body passes directly between a larger body and the observer. As viewed from a particular vantage point, the transiting body appears to move across the face of the larger body, covering a small portion of it." ;
         rdfs:label "Transit"@en ,
                    "Transit"@iri-based .


###  http://visualdataweb.org/SpaceScience/Type_I
:Type_I rdf:type owl:Class ;
        rdfs:subClassOf :supernova ;
        owl:disjointWith :Type_II ;
        rdfs:comment "Definition: star accumulates matter from a nearby neighbor until a runaway nuclear reaction ignites." .


###  http://visualdataweb.org/SpaceScience/Type_II
:Type_II rdf:type owl:Class ;
         rdfs:subClassOf :supernova ;
         rdfs:comment "Definition: star runs out of nuclear fuel and collapses under its own gravity." .


###  http://visualdataweb.org/SpaceScience/USFR_Large
:USFR_Large rdf:type owl:Class ;
            rdfs:subClassOf :USF_Regular_Convex ;
            owl:disjointWith :USFR_Medium .


###  http://visualdataweb.org/SpaceScience/USFR_Medium
:USFR_Medium rdf:type owl:Class ;
             rdfs:subClassOf :USF_Regular_Convex .


###  http://visualdataweb.org/SpaceScience/USF_Regular_Convex
:USF_Regular_Convex rdf:type owl:Class ;
                    rdfs:subClassOf :US_Few_Material ;
                    rdfs:comment """Definition: Objects whose shape is prior know and is convex.

Justification: Classification based on the size of the object. The size is distinguished in three different kinds, small, which is below 10cm, medium, which is between 10cm and 1.5 meter and larger than 1.5 meter in diameter.""" .


###  http://visualdataweb.org/SpaceScience/USMR_Large
:USMR_Large rdf:type owl:Class ;
            rdfs:subClassOf :USM_Regular ;
            owl:disjointWith :USMR_Medium .


###  http://visualdataweb.org/SpaceScience/USMR_Medium
:USMR_Medium rdf:type owl:Class ;
             rdfs:subClassOf :USM_Regular .


###  http://visualdataweb.org/SpaceScience/USM_Regular
:USM_Regular rdf:type owl:Class ;
             rdfs:subClassOf :US_Many_Material ;
             rdfs:comment """Definition: Objects whose shape is prior known with concavities.

Justification: Classification based on the size of the object. The size is distinguished in three different kinds, small, which is below 10cm, medium, which is between 10cm and 1.5 meter and larger than 1.5 meter in diameter.""" .


###  http://visualdataweb.org/SpaceScience/USSR_Large
:USSR_Large rdf:type owl:Class ;
            rdfs:subClassOf :USS_Regular_Convex ;
            owl:disjointWith :USSR_Medium .


###  http://visualdataweb.org/SpaceScience/USSR_Medium
:USSR_Medium rdf:type owl:Class ;
             rdfs:subClassOf :USS_Regular_Convex .


###  http://visualdataweb.org/SpaceScience/USS_Regular_Convex
:USS_Regular_Convex rdf:type owl:Class ;
                    rdfs:subClassOf :US_Single_Material ;
                    rdfs:comment """Definition: Objects whose shape is prior know and is convex.

Justification: Classification based on the size of the object. The size is distinguished in three different kinds, small, which is below 10cm, medium, which is between 10cm and 1.5 meter and larger than 1.5 meter in diameter.""" .


###  http://visualdataweb.org/SpaceScience/US_Few_Material
:US_Few_Material rdf:type owl:Class ;
                 rdfs:subClassOf :U_Spinning ;
                 owl:disjointWith :US_Single_Material ;
                 rdfs:comment """Definitions: Objects that are composed of few materail in between single and many.

Justification: Classification based on the shape of the object.""" .


###  http://visualdataweb.org/SpaceScience/US_Many_Material
:US_Many_Material rdf:type owl:Class ;
                  rdfs:subClassOf :U_Stable ;
                  rdfs:comment """Definition: Objects that are composed of multiple material. 

Justification: Classification based on the shape of the object.""" .


###  http://visualdataweb.org/SpaceScience/US_Single_Material
:US_Single_Material rdf:type owl:Class ;
                    rdfs:subClassOf :U_Spinning ;
                    rdfs:comment """Definition: Objects that are made up of single material.

Justification: Classification based on the shape of the object.""" .


###  http://visualdataweb.org/SpaceScience/UTFI_Medium
:UTFI_Medium rdf:type owl:Class ;
             rdfs:subClassOf :UTF_Irregular ;
             owl:disjointWith :UTFI_Small .


###  http://visualdataweb.org/SpaceScience/UTFI_Small
:UTFI_Small rdf:type owl:Class ;
            rdfs:subClassOf :UTF_Irregular .


###  http://visualdataweb.org/SpaceScience/UTFR_Large
:UTFR_Large rdf:type owl:Class ;
            rdfs:subClassOf :UTF_Regular_Convex ;
            owl:disjointWith :UTFR_Medium .


###  http://visualdataweb.org/SpaceScience/UTFR_Medium
:UTFR_Medium rdf:type owl:Class ;
             rdfs:subClassOf :UTF_Regular_Convex .


###  http://visualdataweb.org/SpaceScience/UTF_Irregular
:UTF_Irregular rdf:type owl:Class ;
               rdfs:subClassOf :UT_Few_Material ;
               owl:disjointWith :UTF_Regular_Convex ;
               rdfs:comment """Definition: Objects whose shape is irregular. 

Justification: Classification based on the size of the object. The size is distinguished in three different kinds, small, which is below 10cm, medium, which is between 10cm and 1.5 meter and larger than 1.5 meter in diameter.""" .


###  http://visualdataweb.org/SpaceScience/UTF_Regular_Convex
:UTF_Regular_Convex rdf:type owl:Class ;
                    rdfs:subClassOf :UT_Few_Material ;
                    rdfs:comment """Definition: Objects whose shape is prior know and is convex.

Justification: Classification based on the size of the object. The size is distinguished in three different kinds, small, which is below 10cm, medium, which is between 10cm and 1.5 meter and larger than 1.5 meter in diameter.""" .


###  http://visualdataweb.org/SpaceScience/UTMR_Large
:UTMR_Large rdf:type owl:Class ;
            rdfs:subClassOf :UTM_Regular ;
            owl:disjointWith :UTMR_Medium .


###  http://visualdataweb.org/SpaceScience/UTMR_Medium
:UTMR_Medium rdf:type owl:Class ;
             rdfs:subClassOf :UTM_Regular .


###  http://visualdataweb.org/SpaceScience/UTM_Regular
:UTM_Regular rdf:type owl:Class ;
             rdfs:subClassOf :UT_Many_Material ;
             rdfs:comment """Definition: Objects whose shape is prior known with concavities.

Justification: Classification based on the size of the object. The size is distinguished in three different kinds, small, which is below 10cm, medium, which is between 10cm and 1.5 meter and larger than 1.5 meter in diameter.""" .


###  http://visualdataweb.org/SpaceScience/UTSI_Medium
:UTSI_Medium rdf:type owl:Class ;
             rdfs:subClassOf :UTS_Irregular ;
             owl:disjointWith :UTSI_Small .


###  http://visualdataweb.org/SpaceScience/UTSI_Small
:UTSI_Small rdf:type owl:Class ;
            rdfs:subClassOf :UTS_Irregular .


###  http://visualdataweb.org/SpaceScience/UTSR_Medium
:UTSR_Medium rdf:type owl:Class ;
             rdfs:subClassOf :UTS_Regular_Convex ;
             owl:disjointWith :UTSR_Small .


###  http://visualdataweb.org/SpaceScience/UTSR_Small
:UTSR_Small rdf:type owl:Class ;
            rdfs:subClassOf :UTS_Regular_Convex .


###  http://visualdataweb.org/SpaceScience/UTS_Irregular
:UTS_Irregular rdf:type owl:Class ;
               rdfs:subClassOf :UT_Single_Material ;
               owl:disjointWith :UTS_Regular_Convex ;
               rdfs:comment """Definition: Objects whose shape is irregular. 

Justification: Classification based on the size of the object. The size is distinguished in three different kinds, small, which is below 10cm, medium, which is between 10cm and 1.5 meter and larger than 1.5 meter in diameter.""" .


###  http://visualdataweb.org/SpaceScience/UTS_Regular_Convex
:UTS_Regular_Convex rdf:type owl:Class ;
                    rdfs:subClassOf :UT_Single_Material ;
                    rdfs:comment """Definition: Objects whose shape is prior know and is convex.

Justification: Classification based on the size of the object. The size is distinguished in three different kinds, small, which is below 10cm, medium, which is between 10cm and 1.5 meter and larger than 1.5 meter in diameter.""" .


###  http://visualdataweb.org/SpaceScience/UT_Few_Material
:UT_Few_Material rdf:type owl:Class ;
                 rdfs:subClassOf :U_Tumbling ;
                 rdfs:comment """Definitions: Objects that are composed of few materail in between single and many. 

Justification: Classification based on the shape of the object.""" .


###  http://visualdataweb.org/SpaceScience/UT_Many_Material
:UT_Many_Material rdf:type owl:Class ;
                  rdfs:subClassOf :U_Tumbling ;
                  rdfs:comment """Definition: Objects that are composed of multiple material. 

Justification: Classification based on the shape of the object.""" .


###  http://visualdataweb.org/SpaceScience/UT_Single_Material
:UT_Single_Material rdf:type owl:Class ;
                    rdfs:subClassOf :U_Tumbling ;
                    rdfs:comment """Definition: Objects that are made up of single material.

Justification: Classification based on the shape of the object.""" .


###  http://visualdataweb.org/SpaceScience/U_Spinning
:U_Spinning rdf:type owl:Class ;
            rdfs:subClassOf :UnControlled_Orbit ;
            rdfs:comment """Definition: Objects that are spinning moderately around one axis.

Justification: Classification based on the number of material used to build the instrument.""" .


###  http://visualdataweb.org/SpaceScience/U_Stable
:U_Stable rdf:type owl:Class ;
          rdfs:subClassOf :UnControlled_Orbit ;
          rdfs:comment """Definition: Objects that are stationary

Justification: Classification based on the number of material used to build the instrument.""" .


###  http://visualdataweb.org/SpaceScience/U_Tumbling
:U_Tumbling rdf:type owl:Class ;
            rdfs:subClassOf :UnControlled_Orbit ;
            rdfs:comment """Definition: Objects that are spinning in irregular manner.

Justification: Classification based on the number of material used to build the instrument.""" .


###  http://visualdataweb.org/SpaceScience/Ultracompact_dwarfs
:Ultracompact_dwarfs rdf:type owl:Class ;
                     rdfs:subClassOf :Low_Luminosity ;
                     rdfs:comment "Definition: has radii as small as 30 light years and has comparatively low surface brightness." .


###  http://visualdataweb.org/SpaceScience/UnControlled_Orbit
:UnControlled_Orbit rdf:type owl:Class ;
                    rdfs:subClassOf :Outer_Space ;
                    rdfs:comment """Definition: Objects whose movement around orbit is not controlled. 

Source: https://amostech.com/TechnicalPapers/2013/Orbital_Debris/JAH.pdf

Justification: Classification is based on the attitude state, i.e, how the attiute of the object is evolving ober time, is it actively stabilized. naturally stable, spinning mderately around one axis or spinning in irregular manner.""" .


###  http://visualdataweb.org/SpaceScience/Visual
:Visual rdf:type owl:Class ;
        rdfs:subClassOf :Binary ;
        rdfs:comment """Definition: distinctly seen with the naked eye through the telescope

Source: Classifying the Cosmos (Book)""" .


###  http://visualdataweb.org/SpaceScience/Warm_Hot_IGM
:Warm_Hot_IGM rdf:type owl:Class ;
              rdfs:subClassOf :G_Gas ;
              rdfs:comment """Definition:The warm–hot intergalactic medium (WHIM) is the sparse, warm-to-hot (105 to 107 K) plasma that cosmologists believe to exist in the spaces between galaxies and to contain 40–50% of the baryonic 'normal matter' in the universe at the current epoch.

Source: https://en.wikipedia.org/wiki/Warm%E2%80%93hot_intergalactic_medium""" .


###  http://visualdataweb.org/SpaceScience/Weak_T_Tauri_stars
:Weak_T_Tauri_stars rdf:type owl:Class ;
                    rdfs:subClassOf :T-Tauri ;
                    rdfs:comment """Definition: Stars that have almost completely lost
their nebulous disk, perhaps because planetesimals—the building
blocks of planets—have formed in the protoplanetary disk

Source: Classifying the Cosmos (Book)""" .


###  http://visualdataweb.org/SpaceScience/White_Dwarf
:White_Dwarf rdf:type owl:Class ;
             rdfs:subClassOf :Evolutionary_Endpoints ;
             rdfs:comment """Definition: A white dwarf is the final stage in the evolution of a star whose
core is less than 1.4 solar masses. 
The original progenitor star may have been as much as 10
solar masses before shedding most of its mass. After burning its
core hydrogen through nuclear fusion, a lower main sequence star
such as our Sun will become a helium-burning red giant (S 7, S
8), producing carbon and oxygen.

Source: Classifying the Cosmos (Book)""" .


###  http://visualdataweb.org/SpaceScience/White_Dwarf_Supernova_Remnant
:White_Dwarf_Supernova_Remnant rdf:type owl:Class ;
                               rdfs:subClassOf :S_Gas ;
                               rdfs:comment """Definition: a white dwarf supernova remnant (Type Ia
in astronomical lingo) results from accretion of material onto a
white dwarf at the Chandrasekhar limit, and its explosion normally
leaves no star behind, or a star in the process of being ejected
from its system. 
White dwarf supernovae remnants show no hydrogen or helium
lines; some show emission lines from the iron group in their later
phases.

Source: Classifying the Cosmos (Book)""" .


###  http://visualdataweb.org/SpaceScience/With_Neuclear_core
:With_Neuclear_core rdf:type owl:Class ;
                    rdfs:subClassOf :High_Luminosity ;
                    owl:disjointWith :Without_Neuclear_core ;
                    rdfs:comment "Definition: Has a neuclear core and are most luminous." .


###  http://visualdataweb.org/SpaceScience/Without_Neuclear_core
:Without_Neuclear_core rdf:type owl:Class ;
                       rdfs:subClassOf :High_Luminosity ;
                       rdfs:comment "Definition: Doesn't have a neuclear core." .


###  http://visualdataweb.org/SpaceScience/supernova
:supernova rdf:type owl:Class ;
           rdfs:subClassOf :Involving_Stars ;
           rdfs:comment """Definition: A supernova is a powerful and luminous stellar explosion. This transient astronomical event occurs during the last evolutionary stages of a massive star or when a white dwarf is triggered into runaway nuclear fusion. 

Source: https://en.wikipedia.org/wiki/Supernova

Justification: Classification based on the manner in which it occurs.""" .


###  http://visualdataweb.org/SpaceScience/G_Filaments_&_Voids
<http://visualdataweb.org/SpaceScience/G_Filaments_&_Voids> rdf:type owl:Class ;
                                                            rdfs:subClassOf :Galaxy_Systems ;
                                                            rdfs:comment """Definition: The existence of structures larger than superclusters, on the scale
of hundreds of millions to billions of light years, was not suspected until four decades ago, when large surveys of galaxy redshifts began to reveal the coherent large-scale structure of the universe.
They constitute the “cosmic web” channeling intergalactic gas (G 14) into galaxies and clusters.""" .


###  http://visualdataweb.org/SpaceScience/Herbig_Ae/Herbig_Ae/Herbig_Ae_Be
<http://visualdataweb.org/SpaceScience/Herbig_Ae/Herbig_Ae/Herbig_Ae_Be> rdf:type owl:Class ;
                                                                         rdfs:subClassOf :Pre-Main_Sequence ;
                                                                         rdfs:comment """Definition: Herbig Ae/Be stars, sometimes referred to as HAeBe stars, are higher mass than T Tauri stars. Their ages range from half a million to
20 million years before the onset of hydrogen nuclear fusion.

Source: Classifying the Cosmos (Book)""" .


###  http://visualdataweb.org/SpaceScience/Proplyd(Disk)
<http://visualdataweb.org/SpaceScience/Proplyd(Disk)> rdf:type owl:Class ;
                                                      rdfs:subClassOf :Protoplanetary ;
                                                      rdfs:comment """Definition: A proplyd, a syllabic abbreviation of an ionized protoplanetary disk, is an externally illuminated photoevaporating disk around a young star. 

Source: https://en.wikipedia.org/wiki/Proplyd""" .


#################################################################
#    General axioms
#################################################################

[ rdf:type owl:AllDisjointClasses ;
  owl:members ( :Advanced
                :Early
                :Intermediate
              )
] .


[ rdf:type owl:AllDisjointClasses ;
  owl:members ( :Association
                :Binary
                :Globular_Cluster
                :Multiple_Star
                :Open_Cluster
                :Population
              )
] .


[ rdf:type owl:AllDisjointClasses ;
  owl:members ( :Asteroid
                :Comet
                :Trans-Neptunian_Objects
              )
] .


[ rdf:type owl:AllDisjointClasses ;
  owl:members ( :Asteroid_Groups
                :Meteroid_streams
                :Planetary_Systems
                :Trans-Neptunian_Systems
              )
] .


[ rdf:type owl:AllDisjointClasses ;
  owl:members ( :Astrometric
                :Photometric
                :Spectroscopic
                :Visual
              )
] .


[ rdf:type owl:AllDisjointClasses ;
  owl:members ( :Aurora
                :Conjunction
                :Ecplise
                :Libration
                :Meteor_Shower
                :Multiple_Objects
                :Single_Objects
                :Solar_Storm
                :Stellar_Occultation
                :Syzygy
                :Transit
              )
] .


[ rdf:type owl:AllDisjointClasses ;
  owl:members ( :Blazar
                :Quasar
                :Radio_Galaxy
                :Seyfert
              )
] .


[ rdf:type owl:AllDisjointClasses ;
  owl:members ( :Bright_Giant
                :Giant
                :Hypergiant
                :Subgiant
                :Supergiant
              )
] .


[ rdf:type owl:AllDisjointClasses ;
  owl:members ( :Circumgalactic
                :Galaxy
                :Galaxy_Systems
                :Intergalactic_Medium
                :Protogalactic
                :Subgalactic
              )
] .


[ rdf:type owl:AllDisjointClasses ;
  owl:members ( :Circumplanetary
                :Interplanetary_Medium
                :Planet
                :Protoplanetary
                :Subplanetary
                :Systems
              )
] .


[ rdf:type owl:AllDisjointClasses ;
  owl:members ( :Circumstellar
                :Interstellar_Medium
                :Protostellar
                :Star
                :Star_Systems
                :Substellar
              )
] .


[ rdf:type owl:AllDisjointClasses ;
  owl:members ( :Classical_KBOs
                :Resonant_KBOs
                :Scattered_KBOs
              )
] .


[ rdf:type owl:AllDisjointClasses ;
  owl:members ( :Cool_Atomic_Cloud
                :Hot_Ionized_Cloud
                :Molecular_Cloud
                :White_Dwarf_Supernova_Remnant
              )
] .


[ rdf:type owl:AllDisjointClasses ;
  owl:members ( :Core_Collapse_Supernova_Remnant
                :Debris_disk
                :Herbig-Haro_Object
                :Nova_Remnant
                :Planetary_Nebula
                :Shell
                :Stellar_Jet
              )
] .


[ rdf:type owl:AllDisjointClasses ;
  owl:members ( :Dust
                :Energetic_Particles
                :Gas
              )
] .


[ rdf:type owl:AllDisjointClasses ;
  owl:members ( :Dwarf_Planet
                :Meteoroid
                :Small_Bodies_of_Solar_System
              )
] .


[ rdf:type owl:AllDisjointClasses ;
  owl:members ( :Earth_Instrument
                :Observational
                :Outer_Space
                :Recording
              )
] .


[ rdf:type owl:AllDisjointClasses ;
  owl:members ( :Elliptical
                :Irregular_Cluster
                :Lenticular
                :Spiral
              )
] .


[ rdf:type owl:AllDisjointClasses ;
  owl:members ( :Evolutionary_Endpoints
                :Main_Sequence
                :Post-Main_Sequence
                :Pre-Main_Sequence
              )
] .


[ rdf:type owl:AllDisjointClasses ;
  owl:members ( :G_Binary
                :G_Cluster
                :G_Group
                :G_Interacting
                :G_Supercluster
                <http://visualdataweb.org/SpaceScience/G_Filaments_&_Voids>
              )
] .


[ rdf:type owl:AllDisjointClasses ;
  owl:members ( :Galactic_Halo
                :Galactic_Jet
                :Galactic_Ring
              )
] .


[ rdf:type owl:AllDisjointClasses ;
  owl:members ( :Galaxy_Merger
                :Involving_Galaxies
                :Involving_Stars
                :Novae
                :supernova
              )
] .


[ rdf:type owl:AllDisjointClasses ;
  owl:members ( :Gas_Giant
                :Ice_Giant
                :Pulsar_Planet
                :Terrestrial
              )
] .


[ rdf:type owl:AllDisjointClasses ;
  owl:members ( :High_Surface_Brightness
                :Low_Surface_Brightness
                :Ultracompact_dwarfs
              )
] .


[ rdf:type owl:AllDisjointClasses ;
  owl:members ( :Intermediate_Black_Hole
                :Stellar_Black_Hole
                :Supermassive_Black_Hole
              )
] .


[ rdf:type owl:AllDisjointClasses ;
  owl:members ( :Kingdom_of_Galaxies
                :Kingdom_of_Planets
                :Kingdom_of_Stars
              )
] .


[ rdf:type owl:AllDisjointClasses ;
  owl:members ( :Mirror_lens
                :Reflective
                :Refracting
              )
] .


[ rdf:type owl:AllDisjointClasses ;
  owl:members ( :Planet_Radiation_Belt
                :Planetary_Ring
                :Plantetary_Satellite
              )
] .


[ rdf:type owl:AllDisjointClasses ;
  owl:members ( :Population_I
                :Population_II
                :Population_III
              )
] .


[ rdf:type owl:AllDisjointClasses ;
  owl:members ( :S_Dust
                :S_Energetic_Particles
                :S_Gas
              )
] .


[ rdf:type owl:AllDisjointClasses ;
  owl:members ( :UT_Few_Material
                :UT_Many_Material
                :UT_Single_Material
              )
] .


[ rdf:type owl:AllDisjointClasses ;
  owl:members ( :U_Spinning
                :U_Stable
                :U_Tumbling
              )
] .


###  Generated by the OWL API (version 4.5.9.2019-02-01T07:24:44Z) https://github.com/owlcs/owlapi
